examples/Common/OwnerMemProof.v
@@ -1,0 +1,352 @@
+Require Import FMapPositive.
+Require Import Coq.PArith.PArith.
+Require Import Coq.Arith.PeanoNat.
+Require Import Coq.Logic.Eqdep.
+Require Import Coq.Logic.Classical.
+Require Import Coq.Relations.Relation_Operators.
+
+Require Import models.EffectSignatures.
+Require Import LinCCAL.
+Require Import LTS.
+Require Import Lang.
+Require Import Semantics.
+Require Import Logics.
+Require Import Assertion.
+Require Import TPSimulationSet.
+Require Import RGILogicSet.
+Require Import SingletonPossibility.
+Require Import CompLinLayer.
+
+Require Import examples.Common.AtomicLTS.
+Require Import examples.Common.Heap.
+Require Import examples.Common.OwnerMemSpec.
+
+
+(** [OwnerMemSpec.OwnerMem] is linearizable from [OwnerMemSpec.PlainMem]
+    with the identity implementation: the owner map is ghost state, so the
+    only content of the proof is that the two memories take the same steps
+    and raise the same errors.  A concrete error is answered by the same
+    abstract error, which discharges the method. *)
+Module OwnerMemProof.
+  Import Reg LinCCALBase LTSSpec Lang Semantics.
+  Import AssertionsSingle SingletonPossibility.
+  Import TPSimulationSet.TPSimulation CompLinLayer.
+  Import AtomicLTS OwnerMemSpec PlainMem OwnerMem.
+  Import (coercions, canonicals, notations) Sig.
+  Import (notations) LinCCAL.
+  Module SetLogic := RGILogicSet.RGILogic.
+  Import SetLogic.
+
+  Open Scope prog_scope.
+  Open Scope assertion_scope.
+  Open Scope rg_relation_scope.
+
+  Section Proof.
+    Context {X : Type}.
+
+    Definition E : layer_interface := @PlainMemLayer.L X.
+    Definition F : layer_interface := @OwnerMemLayer.L X.
+
+    Definition owner_mem_impl : ModuleImpl (li_sig E) (li_sig F) :=
+      fun m _ => m >= r => Ret r.
+
+    Definition single_state :=
+      @SinglePossState.ProofStateSingle _ _ (li_lts E) (li_lts F).
+    Definition assertion := @Assertion single_state.
+    Definition rg_relation :=
+      @AssertionsSingle.A.RGRelation _ _ (li_lts E) (li_lts F).
+
+    (** The abstract state is the concrete one plus the owner map. *)
+    Definition state_rel (c : State (li_lts E)) (a : State (li_lts F)) : Prop :=
+      match c, a with
+      | Idle h, Idle om => om_heap om = h
+      | Pending h t p, Pending om t' q => t = t' /\ p = q /\ om_heap om = h
+      | _, _ => False
+      end.
+
+    Definition I : assertion := fun s => state_rel (σ s) (ρ s).
+
+    Definition G (t : tid) : rg_relation := fun s s' =>
+      forall t', t <> t' -> TMap.find t' (π s) = TMap.find t' (π s').
+    Definition R (t : tid) : rg_relation := fun s s' =>
+      TMap.find t (π s) = TMap.find t (π s').
+
+    Lemma I_stable t : Stable (R t) I I.
+    Proof. apply Stable_invariant. Qed.
+
+    Lemma ALin_stable t ls : Stable (R t) I (ALin t ls).
+    Proof. intros s [[pre [Hlin Hπ]] _]. unfold ALin in *. congruence. Qed.
+
+    Create HintDb stableDB.
+    #[local] Hint Resolve I_stable ALin_stable : stableDB.
+
+    Lemma source_valid_rg t : forall s s', R t s s' -> I s' ->
+      TMap.find t (π s) = None <-> TMap.find t (π s') = None.
+    Proof. intros s s' Hπ _. unfold R in Hπ. rewrite Hπ. tauto. Qed.
+
+    Lemma source_rg_compatible t1 t2 : t1 <> t2 -> forall s s',
+      (G t1 s s' \/ (GINV t1 s s' \/ GRET t1 s s') \/ GId s s') ->
+      R t2 s s'.
+    Proof.
+      intros Hneq s s' [HG | [[Hinv | Hret] | Hid]]; unfold R.
+      - apply HG. exact Hneq.
+      - destruct Hinv as [f [_ [_ [_ Hπ]]]]. rewrite Hπ, TMap.gso; auto.
+      - destruct Hret as [f [ret [_ [_ [_ Hπ]]]]]. rewrite Hπ, TMap.gro; auto.
+      - unfold GId in Hid. subst. reflexivity.
+    Qed.
+
+    (** * Steps of the two memories *)
+
+    Definition oread_result (ev : @ThreadEvent (EOMem X)) : option X :=
+      match te_ev ev with
+      | ResEv op ret =>
+          match op return (Sig.ar op -> option X) with
+          | oread _ => fun v => Some v
+          | _ => fun _ => None
+          end ret
+      | InvEv _ => None
+      end.
+
+    Definition omalloc_result (ev : @ThreadEvent (EOMem X)) : option Addr :=
+      match te_ev ev with
+      | ResEv op ret =>
+          match op return (Sig.ar op -> option Addr) with
+          | omalloc _ => fun l => Some l
+          | _ => fun _ => None
+          end ret
+      | InvEv _ => None
+      end.
+
+    Definition ocas_result (ev : @ThreadEvent (EOMem X)) : option bool :=
+      match te_ev ev with
+      | ResEv op ret =>
+          match op return (Sig.ar op -> option bool) with
+          | ocas _ _ _ => fun b => Some b
+          | _ => fun _ => None
+          end ret
+      | InvEv _ => None
+      end.
+
+    Ltac crush :=
+      repeat match goal with
+      | H : {| te_tid := _; te_ev := _ |} = {| te_tid := _; te_ev := _ |} |- _ =>
+          first [ apply (f_equal oread_result) in H; discriminate H
+                | apply (f_equal omalloc_result) in H; discriminate H
+                | apply (f_equal ocas_result) in H; discriminate H
+                | injection H; clear H; intros ]
+      | H : InvEv _ = ResEv _ _ |- _ => discriminate H
+      | H : ResEv _ _ = InvEv _ |- _ => discriminate H
+      | H : InvEv _ = InvEv _ |- _ => injection H; clear H; intros
+      | H : ResEv _ _ = ResEv _ _ |- _ => injection H; clear H; intros
+      | H : omalloc _ = omalloc _ |- _ => injection H; clear H; intros
+      | H : oread _ = oread _ |- _ => injection H; clear H; intros
+      | H : owrite _ _ = owrite _ _ |- _ => injection H; clear H; intros
+      | H : ocas _ _ _ = ocas _ _ _ |- _ => injection H; clear H; intros
+      | H : existT _ _ _ = existT _ _ _ |- _ => apply inj_pair2 in H
+      | H : ?x = ?x |- _ => clear H
+      | H : ?x = ?y |- _ => is_var y; subst y
+      | H : ?x = ?y |- _ => is_var x; subst x
+      end;
+      try discriminate; try congruence.
+
+    (** Precondition of an invocation, shared by both memories. *)
+    Definition inv_ok (m : Sig.op (EOMem X)) (h : @Heap X) : Prop :=
+      match m with
+      | omalloc _ => True
+      | oread l => h l <> None
+      | owrite l _ => h l <> None
+      | ocas l _ _ => h l <> None
+      end.
+
+    Lemma plain_inv_shape t m c c' :
+      Step (li_lts E) {| te_tid := t; te_ev := InvEv m |} c c' ->
+      exists h, c = Idle h /\ c' = Pending h t m /\ inv_ok m h.
+    Proof.
+      intros Hstep. inversion Hstep; subst; crush.
+      inversion Hstep0; subst; crush; eexists; repeat split; simpl; auto.
+    Qed.
+
+    Lemma owner_inv_step t m (om : OMemState X) :
+      inv_ok m (om_heap om) ->
+      Step (li_lts F) {| te_tid := t; te_ev := InvEv m |} (Idle om) (Pending om t m).
+    Proof.
+      intros Hok. apply step_inv. destruct m; simpl in Hok.
+      - eapply step_alloc_inv; reflexivity.
+      - eapply step_read_inv; [reflexivity|exact Hok].
+      - eapply step_write_inv; [reflexivity|exact Hok].
+      - eapply step_cas_inv; [reflexivity|exact Hok].
+    Qed.
+
+    (** Every concrete response has an abstract counterpart with the same
+        heap. *)
+    Lemma plain_res_matches t m r (h h' : @Heap X) (om : OMemState X) :
+      om_heap om = h ->
+      StepPlain {| te_tid := t; te_ev := ResEv m r |} h h' ->
+      exists om', om_heap om' = h' /\
+        StepOMem {| te_tid := t; te_ev := ResEv m r |} om om'.
+    Proof.
+      intros Hh Hstep. subst h. inversion Hstep; subst; crush.
+      - match goal with |- context [heap_update ?l ?v _] => exists (om_alloc t l v om) end.
+        split; [reflexivity|]. eapply step_alloc_res; [reflexivity|assumption].
+      - exists om. split; [reflexivity|]. eapply step_read_res; [reflexivity|assumption].
+      - match goal with |- context [heap_update ?l ?v _] => exists (om_write l v om) end.
+        split; [reflexivity|]. eapply step_write_res; [reflexivity|assumption].
+      - match goal with |- context [heap_update ?l ?v _] => exists (om_write l v om) end.
+        split; [reflexivity|]. eapply step_cas_res_succ; [reflexivity|assumption].
+      - exists om. split; [reflexivity|].
+        eapply step_cas_res_fail; [reflexivity|eassumption|assumption].
+    Qed.
+
+    Lemma plain_res_shape t m r c c' :
+      Step (li_lts E) {| te_tid := t; te_ev := ResEv m r |} c c' ->
+      exists h h', c = Pending h t m /\ c' = Idle h' /\
+        StepPlain {| te_tid := t; te_ev := ResEv m r |} h h'.
+    Proof.
+      intros Hstep. inversion Hstep; subst; crush. eauto.
+    Qed.
+
+    (** * Errors *)
+
+    Lemma concrete_error_refines t m c a :
+      state_rel c a ->
+      Error (li_lts E) {| te_tid := t; te_ev := InvEv m |} c ->
+      Error (li_lts F) {| te_tid := t; te_ev := InvEv m |} a.
+    Proof.
+      unfold state_rel. destruct c as [h | h tp p], a as [om | om tq q];
+        simpl; try contradiction.
+      - intros Hh Herr. subst h. inversion Herr; subst; crush.
+        + eapply error_read_undefined; eauto.
+        + eapply error_write_undefined; eauto.
+        + eapply error_cas_undefined; eauto.
+      - intros [Ht [Hp Hh]] Herr. subst tq q h. inversion Herr; subst; crush.
+        eapply error_write_racy; eauto.
+    Qed.
+
+    Lemma no_error_or_abstract_error t m :
+      ⊨ I //\\ ALin t (ls_inv m) ==>>
+        (I //\\ ALin t (ls_inv m) //\\ ANoError {| te_tid := t; te_ev := InvEv m |})
+        \\// APError.
+    Proof.
+      intros s [HI Hlin].
+      destruct (classic (Error (li_lts E) {| te_tid := t; te_ev := InvEv m |} (σ s)))
+        as [Herr | Hno].
+      - right. apply rt_step. eapply (ps_error t m); [|exact Hlin].
+        apply concrete_error_refines with (c := σ s); assumption.
+      - left. split; [exact HI|]. split; [exact Hlin|exact Hno].
+    Qed.
+
+    Lemma lift_perror (P P' : assertion) :
+      (⊨ P ==>> P' \\// APError) ->
+      ⊨ lift_assert P ==>> lift_assert P' \\// AssertionsSet.APError.
+    Proof.
+      intros Himpl s [x [Hview HP]].
+      destruct (Himpl x HP) as [HP'|Herr].
+      - left. exists x. auto.
+      - right. eapply AssertionsSet.APErrorSome.
+        + apply singleton_view_member. exact Hview.
+        + exact Herr.
+    Qed.
+
+    (** * Possibility updates *)
+
+    Lemma inv_update t m :
+      PUpdate (G t) {| te_tid := t; te_ev := InvEv m |}
+        (I //\\ ALin t (ls_inv m) //\\ ANoError {| te_tid := t; te_ev := InvEv m |})
+        (I //\\ ALin t (ls_lini m)).
+    Proof.
+      intros c a p [HI [Hlin _]] c' Hstep.
+      destruct (plain_inv_shape _ _ _ _ Hstep) as [h [-> [-> Hok]]].
+      unfold I, state_rel in HI. simpl in HI.
+      destruct a as [om | om tq q]; [|contradiction]. subst h.
+      exists (Pending om t m), (TMap.add t (ls_lini m) p). split.
+      { apply rt_step. apply (ps_inv t m); [|exact Hlin].
+        apply owner_inv_step. exact Hok. }
+      split.
+      - split; [unfold I, state_rel; simpl; auto|].
+        unfold ALin. simpl. apply TMap.gss.
+      - intros t' Hne. simpl. rewrite TMap.gso; auto.
+    Qed.
+
+    Lemma res_update t m r :
+      PUpdate (G t) {| te_tid := t; te_ev := ResEv m r |}
+        (I //\\ ALin t (ls_lini m))
+        (I //\\ ALin t (ls_linr m r)).
+    Proof.
+      intros c a p [HI Hlin] c' Hstep.
+      destruct (plain_res_shape _ _ _ _ _ Hstep) as [h [h' [-> [-> Hres]]]].
+      unfold I, state_rel in HI. simpl in HI.
+      destruct a as [om | om tq q]; [contradiction|].
+      destruct HI as [<- [<- Hh]].
+      destruct (plain_res_matches _ _ _ _ _ _ Hh Hres) as [om' [Hh' Hstep']].
+      exists (Idle om'), (TMap.add t (ls_linr m r) p). split.
+      { apply rt_step. apply (ps_ret t m r); [|exact Hlin].
+        apply step_res. exact Hstep'. }
+      split.
+      - split; [unfold I, state_rel; simpl; exact Hh'|].
+        unfold ALin. simpl. apply TMap.gss.
+      - intros t' Hne. simpl. rewrite TMap.gso; auto.
+    Qed.
+
+    (** * The layer *)
+
+    Program Definition MOwnerMem : layer_implementation_simulation E F :=
+    {| li_impl := owner_mem_impl |}.
+    Next Obligation.
+      eapply SetLogic.soundness
+        with (R := fun t => lift_relation (R t))
+             (G := fun t => lift_relation (G t))
+             (I := lift_assert I).
+      { intros t. eapply lift_valid_rgi. apply source_valid_rg. }
+      {
+        intros t1 t2 Hneq s s' Hrel.
+        eapply lift_parallel_compat; [exact Hneq| |exact Hrel].
+        apply source_rg_compatible; exact Hneq.
+      }
+      {
+        intros t m.
+        exists (lift_assert (I //\\ ALin t (ls_inv m))).
+        exists (fun r => lift_assert (I //\\ ALin t (ls_linr m r))).
+        constructor.
+        - intros s Hcompose.
+          eapply (lift_ginv_compose t m I (I //\\ ALin t (ls_inv m)));
+            [|exact Hcompose].
+          intros out [pre [HI [Hσ [Hρ [Hnone Hπ]]]]].
+          destruct pre as [σp ρp πp], out as [σo ρo πo]. simpl in *. subst.
+          split; [exact HI|]. unfold ALin. simpl. apply TMap.gss.
+        - intros s Hlift. eapply lift_impl; [|exact Hlift].
+          apply ConjLeftImpl. apply ImplRefl.
+        - apply lift_stable. solve_conj_stable stableDB.
+        - intros r s Hcompose.
+          eapply (lift_gret_compose t m r (I //\\ ALin t (ls_linr m r)) I);
+            [|exact Hcompose].
+          intros out [pre [[HI _] [Hσ [Hρ _]]]].
+          destruct pre as [σp ρp πp], out as [σo ρo πo]. simpl in *. subst.
+          exact HI.
+        - intros r σ0 Δ0 Hpost ρ0 π0 Hposs.
+          eapply (lift_post_lin (I //\\ ALin t (ls_linr m r)) t (ls_linr m r));
+            [|exact Hpost|exact Hposs].
+          intros x [_ Hlin]. exact Hlin.
+        - simpl. unfold owner_mem_impl.
+          eapply SetLogic.provable_perror.
+          { apply lift_perror. apply no_error_or_abstract_error. }
+          eapply singleton_provable_vis_safe with
+            (P' := I //\\ ALin t (ls_lini m))
+            (Q' := fun r => I //\\ ALin t (ls_linr m r)).
+          + intros s [_ [_ H]]. exact H.
+          + intros s [HI _]. exact HI.
+          + intros r s [HI _]. exact HI.
+          + solve_conj_stable stableDB.
+          + intros r. solve_conj_stable stableDB.
+          + apply inv_update.
+          + intros r. apply res_update.
+          + intros r. singleton_ret_safe;
+              [apply ImplRefl|intros s [HI _]; exact HI|solve_conj_stable stableDB].
+      }
+      { apply lift_initial. unfold I, state_rel. reflexivity. }
+    Defined.
+
+    Definition MOwnerMemLinearizable := LISim2LILin MOwnerMem.
+  End Proof.
+
+  Print Assumptions MOwnerMem.
+End OwnerMemProof.
