examples/TSStack/NodeMemProof.v
@@ -1,0 +1,2617 @@
+Require Import FMapPositive.
+Require Import Coq.PArith.PArith.
+Require Import Coq.Arith.PeanoNat.
+Require Import Coq.Logic.Eqdep.
+Require Import Coq.Logic.FunctionalExtensionality.
+Require Import Coq.Logic.Classical.
+Require Import Coq.Relations.Relation_Operators.
+Require Import Lia.
+
+Require Import models.EffectSignatures.
+Require Import LinCCAL.
+Require Import LTS.
+Require Import Lang.
+Require Import Semantics.
+Require Import Logics.
+Require Import Assertion.
+Require Import TPSimulationSet.
+Require Import RGILogicSet.
+Require Import SingletonPossibility.
+Require Import CompLinLayer.
+
+Require Import examples.Common.AtomicLTS.
+Require Import examples.Common.Heap.
+Require Import examples.Common.OwnerMemSpec.
+Require Import examples.Common.OwnerMemProof.
+Require Import examples.TSStack.TimestampSpec.
+Require Import examples.TSStack.NodeMemSpec.
+Require Import examples.TSStack.NodeMem.
+
+
+Module NodeMemProof.
+  Import Reg LinCCALBase LTSSpec Lang Semantics.
+  Import AssertionsSingle SingletonPossibility.
+  Import TPSimulationSet.TPSimulation CompLinLayer.
+  Import AtomicLTS OwnerMemSpec OwnerMem OwnerMemProof TimestampSpec NodeMemSpec NodeMemImpl.
+  Import (coercions, canonicals, notations) Sig.
+  Import (notations) LinCCAL.
+  Import (canonicals) Sig.Plus.
+  Module SetLogic := RGILogicSet.RGILogic.
+  Import SetLogic.
+
+  Open Scope prog_scope.
+  Open Scope assertion_scope.
+  Open Scope rg_relation_scope.
+
+  Section Proof.
+    Context {A : Type}.
+
+    Definition E : layer_interface := @NodeMemImpl.E A.
+    Definition F : layer_interface := @NodeMemImpl.F A.
+
+    Definition single_state :=
+      @SinglePossState.ProofStateSingle _ _ (li_lts E) (li_lts F).
+    Definition assertion := @Assertion single_state.
+    Definition rg_relation :=
+      @AssertionsSingle.A.RGRelation _ _ (li_lts E) (li_lts F).
+
+    (** * Views of the concrete state *)
+
+    Definition rec_control := @AState (EOMem (@NodeRec)) (OMemState (@NodeRec)).
+    Definition val_control := @AState (EOMem A) (OMemState A).
+    Definition ts_control := @AState (EOMem TS) (OMemState TS).
+    Definition next_control := @AState (EOMem Ptr) (OMemState Ptr).
+    Definition taken_control := @AState (EOMem bool) (OMemState bool).
+
+    Definition rec_c (c : State (li_lts E)) : rec_control := fst (fst (fst (fst c))).
+    Definition val_c (c : State (li_lts E)) : val_control := snd (fst (fst (fst c))).
+    Definition ts_c (c : State (li_lts E)) : ts_control := snd (fst (fst c)).
+    Definition next_c (c : State (li_lts E)) : next_control := snd (fst c).
+    Definition taken_c (c : State (li_lts E)) : taken_control := snd c.
+
+    Definition rec_h (c : State (li_lts E)) : @Heap (@NodeRec) :=
+      om_heap (state (rec_c c)).
+    Definition val_h (c : State (li_lts E)) : @Heap A := om_heap (state (val_c c)).
+    Definition val_o (c : State (li_lts E)) : @Heap tid := om_owner (state (val_c c)).
+    Definition ts_h (c : State (li_lts E)) : @Heap TS := om_heap (state (ts_c c)).
+    Definition ts_o (c : State (li_lts E)) : @Heap tid := om_owner (state (ts_c c)).
+    Definition next_h (c : State (li_lts E)) : @Heap Ptr := om_heap (state (next_c c)).
+    Definition next_o (c : State (li_lts E)) : @Heap tid := om_owner (state (next_c c)).
+    Definition taken_h (c : State (li_lts E)) : @Heap bool := om_heap (state (taken_c c)).
+    Definition taken_o (c : State (li_lts E)) : @Heap tid := om_owner (state (taken_c c)).
+
+    Definition mk (rc : rec_control) (vc : val_control) (tc : ts_control)
+        (nc : next_control) (kc : taken_control) : State (li_lts E) :=
+      pair (pair (pair (pair rc vc) tc) nc) kc.
+
+    Lemma state_mk (c : State (li_lts E)) :
+      c = mk (rec_c c) (val_c c) (ts_c c) (next_c c) (taken_c c).
+    Proof.
+      destruct c as [[[[rc vc] tc] nc] kc]. reflexivity.
+    Qed.
+
+    (** Projections of the record. *)
+    Definition rec_val (r : @NodeRec) : Addr := fst (fst (fst r)).
+    Definition rec_ts (r : @NodeRec) : Addr := snd (fst (fst r)).
+    Definition rec_taken (r : @NodeRec) : Addr := snd (fst r).
+    Definition rec_next (r : @NodeRec) : Addr := snd r.
+
+    Definition node_val (n : @Node A) : A := fst (fst (fst n)).
+    Definition node_ts (n : @Node A) : TS := snd (fst (fst n)).
+    Definition node_taken (n : @Node A) : bool := snd (fst n).
+    Definition node_next (n : @Node A) : Ptr := snd n.
+
+    (** * Steps of one component memory *)
+
+    Section OneMemory.
+      Context {X : Type}.
+
+      Definition oread_result (ev : @ThreadEvent (EOMem X)) : option X :=
+        match te_ev ev with
+        | ResEv op ret =>
+            match op return (Sig.ar op -> option X) with
+            | oread _ => fun v => Some v
+            | _ => fun _ => None
+            end ret
+        | InvEv _ => None
+        end.
+
+      Definition omalloc_result (ev : @ThreadEvent (EOMem X)) : option Addr :=
+        match te_ev ev with
+        | ResEv op ret =>
+            match op return (Sig.ar op -> option Addr) with
+            | omalloc _ => fun l => Some l
+            | _ => fun _ => None
+            end ret
+        | InvEv _ => None
+        end.
+
+      Definition ocas_result (ev : @ThreadEvent (EOMem X)) : option bool :=
+        match te_ev ev with
+        | ResEv op ret =>
+            match op return (Sig.ar op -> option bool) with
+            | ocas _ _ _ => fun b => Some b
+            | _ => fun _ => None
+            end ret
+        | InvEv _ => None
+        end.
+
+      Ltac crush_omem_step :=
+        repeat match goal with
+        | H : {| te_tid := _; te_ev := _ |} = {| te_tid := _; te_ev := _ |} |- _ =>
+            first [ apply (f_equal oread_result) in H; discriminate H
+                  | apply (f_equal omalloc_result) in H; discriminate H
+                  | apply (f_equal ocas_result) in H; discriminate H
+                  | injection H; clear H; intros ]
+        | H : InvEv _ = ResEv _ _ |- _ => discriminate H
+        | H : ResEv _ _ = InvEv _ |- _ => discriminate H
+        | H : InvEv _ = InvEv _ |- _ => injection H; clear H; intros
+        | H : ResEv _ _ = ResEv _ _ |- _ => injection H; clear H; intros
+        | H : omalloc _ = omalloc _ |- _ => injection H; clear H; intros
+        | H : oread _ = oread _ |- _ => injection H; clear H; intros
+        | H : owrite _ _ = owrite _ _ |- _ => injection H; clear H; intros
+        | H : ocas _ _ _ = ocas _ _ _ |- _ => injection H; clear H; intros
+        | H : existT _ _ _ = existT _ _ _ |- _ => apply inj_pair2 in H
+        | H : ?x = ?x |- _ => clear H
+        | H : ?x = ?y |- _ => is_var y; subst y
+        | H : ?x = ?y |- _ => is_var x; subst x
+        end;
+        try discriminate; try congruence.
+
+      Lemma omem_inv_shape t op (c c' : @AState (EOMem X) (OMemState X)) :
+        Step (@VOMem X) {| te_tid := t; te_ev := InvEv op |} c c' ->
+        exists s, c = Idle s /\ c' = Pending s t op.
+      Proof.
+        intros Hstep. inversion Hstep; subst; crush_omem_step.
+        inversion Hstep0; subst; crush_omem_step; eauto.
+      Qed.
+
+      Lemma omem_alloc_res_shape t v l (c c' : @AState (EOMem X) (OMemState X)) :
+        Step (@VOMem X) {| te_tid := t; te_ev := ResEv (omalloc v) l |} c c' ->
+        exists s, c = Pending s t (omalloc v) /\ om_heap s l = None /\
+          c' = Idle (om_alloc t l v s).
+      Proof.
+        intros Hstep. inversion Hstep; subst; crush_omem_step.
+        inversion Hstep0; subst; crush_omem_step. eauto.
+      Qed.
+
+      Lemma omem_read_res_shape t l v (c c' : @AState (EOMem X) (OMemState X)) :
+        Step (@VOMem X) {| te_tid := t; te_ev := ResEv (oread l) v |} c c' ->
+        exists s, c = Pending s t (oread l) /\ om_heap s l = Some v /\ c' = Idle s.
+      Proof.
+        intros Hstep. inversion Hstep; subst; crush_omem_step.
+        inversion Hstep0; subst; crush_omem_step. eauto.
+      Qed.
+
+      Lemma omem_write_res_shape t l v (c c' : @AState (EOMem X) (OMemState X)) :
+        Step (@VOMem X) {| te_tid := t; te_ev := ResEv (owrite l v) tt |} c c' ->
+        exists s, c = Pending s t (owrite l v) /\ om_heap s l <> None /\
+          c' = Idle (om_write l v s).
+      Proof.
+        intros Hstep. inversion Hstep; subst; crush_omem_step.
+        inversion Hstep0; subst; crush_omem_step. eauto.
+      Qed.
+
+      Lemma omem_cas_true_shape t l v w (c c' : @AState (EOMem X) (OMemState X)) :
+        Step (@VOMem X) {| te_tid := t; te_ev := ResEv (ocas l v w) true |} c c' ->
+        exists s, c = Pending s t (ocas l v w) /\ om_heap s l = Some v /\
+          c' = Idle (om_write l w s).
+      Proof.
+        intros Hstep. inversion Hstep; subst; crush_omem_step.
+        inversion Hstep0; subst; crush_omem_step. eauto.
+      Qed.
+
+      Lemma omem_cas_false_shape t l v w (c c' : @AState (EOMem X) (OMemState X)) :
+        Step (@VOMem X) {| te_tid := t; te_ev := ResEv (ocas l v w) false |} c c' ->
+        exists s u, c = Pending s t (ocas l v w) /\ om_heap s l = Some u /\
+          u <> v /\ c' = Idle s.
+      Proof.
+        intros Hstep. inversion Hstep; subst; crush_omem_step.
+        inversion Hstep0; subst; crush_omem_step. eauto 10.
+      Qed.
+
+      (** Errors of one memory. *)
+      Lemma omem_alloc_no_error t v (c : @AState (EOMem X) (OMemState X)) :
+        ~ Error (@VOMem X) {| te_tid := t; te_ev := InvEv (omalloc v) |} c.
+      Proof.
+        intros Herr. inversion Herr; subst; crush_omem_step.
+      Qed.
+
+      Lemma omem_read_no_error t l (c : @AState (EOMem X) (OMemState X)) :
+        om_heap (state c) l <> None ->
+        ~ Error (@VOMem X) {| te_tid := t; te_ev := InvEv (oread l) |} c.
+      Proof.
+        intros Hdef Herr. inversion Herr; subst; crush_omem_step;
+        simpl in Hdef; congruence.
+      Qed.
+
+      Lemma omem_cas_no_error t l v w (c : @AState (EOMem X) (OMemState X)) :
+        om_heap (state c) l <> None ->
+        ~ Error (@VOMem X) {| te_tid := t; te_ev := InvEv (ocas l v w) |} c.
+      Proof.
+        intros Hdef Herr. inversion Herr; subst; crush_omem_step;
+        simpl in Hdef; congruence.
+      Qed.
+
+      Lemma omem_write_no_error t l v (c : @AState (EOMem X) (OMemState X)) :
+        om_heap (state c) l <> None ->
+        (forall s t' v', c = Pending s t' (owrite l v') -> t = t') ->
+        ~ Error (@VOMem X) {| te_tid := t; te_ev := InvEv (owrite l v) |} c.
+      Proof.
+        intros Hdef Hrace Herr. inversion Herr; subst; crush_omem_step;
+        simpl in Hdef; try congruence.
+        match goal with
+        | Hne : ?t <> ?t' |- False => apply Hne; eapply Hrace; reflexivity
+        end.
+      Qed.
+    End OneMemory.
+
+    (** * Projecting tensor steps to one component *)
+
+    Definition rec_ev (ev : @Event (EOMem (@NodeRec))) : @Event (li_sig E) :=
+      match ev with
+      | InvEv m => InvEv (in_rec m)
+      | ResEv m r => ResEv (in_rec m) r
+      end.
+    Definition val_ev (ev : @Event (EOMem A)) : @Event (li_sig E) :=
+      match ev with
+      | InvEv m => InvEv (in_val m)
+      | ResEv m r => ResEv (in_val m) r
+      end.
+    Definition ts_ev (ev : @Event (EOMem TS)) : @Event (li_sig E) :=
+      match ev with
+      | InvEv m => InvEv (in_ts m)
+      | ResEv m r => ResEv (in_ts m) r
+      end.
+    Definition next_ev (ev : @Event (EOMem Ptr)) : @Event (li_sig E) :=
+      match ev with
+      | InvEv m => InvEv (in_next m)
+      | ResEv m r => ResEv (in_next m) r
+      end.
+    Definition taken_ev (ev : @Event (EOMem bool)) : @Event (li_sig E) :=
+      match ev with
+      | InvEv m => InvEv (in_taken m)
+      | ResEv m r => ResEv (in_taken m) r
+      end.
+
+    Lemma step_rec t ev c c' :
+      Step (li_lts E) {| te_tid := t; te_ev := rec_ev ev |} c c' ->
+      Step (@VOMem (@NodeRec)) {| te_tid := t; te_ev := ev |} (rec_c c) (rec_c c') /\
+      val_c c' = val_c c /\ ts_c c' = ts_c c /\ next_c c' = next_c c /\
+      taken_c c' = taken_c c.
+    Proof.
+      destruct c as [[[[rc vc] tc] nc] kc], c' as [[[[rc' vc'] tc'] nc'] kc'].
+      destruct ev; simpl; unfold in_rec; simpl; intros H;
+      decompose [and] H;
+      repeat match goal with
+      | H : pair _ _ = pair _ _ |- _ => injection H; clear H; intros
+      end; subst; auto.
+    Qed.
+
+    Lemma step_val t ev c c' :
+      Step (li_lts E) {| te_tid := t; te_ev := val_ev ev |} c c' ->
+      Step (@VOMem A) {| te_tid := t; te_ev := ev |} (val_c c) (val_c c') /\
+      rec_c c' = rec_c c /\ ts_c c' = ts_c c /\ next_c c' = next_c c /\
+      taken_c c' = taken_c c.
+    Proof.
+      destruct c as [[[[rc vc] tc] nc] kc], c' as [[[[rc' vc'] tc'] nc'] kc'].
+      destruct ev; simpl; unfold in_val; simpl; intros H;
+      decompose [and] H;
+      repeat match goal with
+      | H : pair _ _ = pair _ _ |- _ => injection H; clear H; intros
+      end; subst; auto.
+    Qed.
+
+    Lemma step_ts t ev c c' :
+      Step (li_lts E) {| te_tid := t; te_ev := ts_ev ev |} c c' ->
+      Step (@VOMem TS) {| te_tid := t; te_ev := ev |} (ts_c c) (ts_c c') /\
+      rec_c c' = rec_c c /\ val_c c' = val_c c /\ next_c c' = next_c c /\
+      taken_c c' = taken_c c.
+    Proof.
+      destruct c as [[[[rc vc] tc] nc] kc], c' as [[[[rc' vc'] tc'] nc'] kc'].
+      destruct ev; simpl; unfold in_ts; simpl; intros H;
+      decompose [and] H;
+      repeat match goal with
+      | H : pair _ _ = pair _ _ |- _ => injection H; clear H; intros
+      end; subst; auto.
+    Qed.
+
+    Lemma step_next t ev c c' :
+      Step (li_lts E) {| te_tid := t; te_ev := next_ev ev |} c c' ->
+      Step (@VOMem Ptr) {| te_tid := t; te_ev := ev |} (next_c c) (next_c c') /\
+      rec_c c' = rec_c c /\ val_c c' = val_c c /\ ts_c c' = ts_c c /\
+      taken_c c' = taken_c c.
+    Proof.
+      destruct c as [[[[rc vc] tc] nc] kc], c' as [[[[rc' vc'] tc'] nc'] kc'].
+      destruct ev; simpl; unfold in_next; simpl; intros H;
+      decompose [and] H;
+      repeat match goal with
+      | H : pair _ _ = pair _ _ |- _ => injection H; clear H; intros
+      end; subst; auto.
+    Qed.
+
+    Lemma step_taken t ev c c' :
+      Step (li_lts E) {| te_tid := t; te_ev := taken_ev ev |} c c' ->
+      Step (@VOMem bool) {| te_tid := t; te_ev := ev |} (taken_c c) (taken_c c') /\
+      rec_c c' = rec_c c /\ val_c c' = val_c c /\ ts_c c' = ts_c c /\
+      next_c c' = next_c c.
+    Proof.
+      destruct c as [[[[rc vc] tc] nc] kc], c' as [[[[rc' vc'] tc'] nc'] kc'].
+      destruct ev; simpl; unfold in_taken; simpl; intros H;
+      decompose [and] H;
+      repeat match goal with
+      | H : pair _ _ = pair _ _ |- _ => injection H; clear H; intros
+      end; subst; auto.
+    Qed.
+
+    Lemma error_rec t ev c :
+      Error (li_lts E) {| te_tid := t; te_ev := rec_ev ev |} c ->
+      Error (@VOMem (@NodeRec)) {| te_tid := t; te_ev := ev |} (rec_c c).
+    Proof.
+      destruct c as [[[[rc vc] tc] nc] kc]. destruct ev; simpl; unfold in_rec; auto.
+    Qed.
+
+    Lemma error_val t ev c :
+      Error (li_lts E) {| te_tid := t; te_ev := val_ev ev |} c ->
+      Error (@VOMem A) {| te_tid := t; te_ev := ev |} (val_c c).
+    Proof.
+      destruct c as [[[[rc vc] tc] nc] kc]. destruct ev; simpl; unfold in_val; auto.
+    Qed.
+
+    Lemma error_ts t ev c :
+      Error (li_lts E) {| te_tid := t; te_ev := ts_ev ev |} c ->
+      Error (@VOMem TS) {| te_tid := t; te_ev := ev |} (ts_c c).
+    Proof.
+      destruct c as [[[[rc vc] tc] nc] kc]. destruct ev; simpl; unfold in_ts; auto.
+    Qed.
+
+    Lemma error_next t ev c :
+      Error (li_lts E) {| te_tid := t; te_ev := next_ev ev |} c ->
+      Error (@VOMem Ptr) {| te_tid := t; te_ev := ev |} (next_c c).
+    Proof.
+      destruct c as [[[[rc vc] tc] nc] kc]. destruct ev; simpl; unfold in_next; auto.
+    Qed.
+
+    Lemma error_taken t ev c :
+      Error (li_lts E) {| te_tid := t; te_ev := taken_ev ev |} c ->
+      Error (@VOMem bool) {| te_tid := t; te_ev := ev |} (taken_c c).
+    Proof.
+      destruct c as [[[[rc vc] tc] nc] kc]. destruct ev; simpl; unfold in_taken; auto.
+    Qed.
+
+    (** * The invariant *)
+
+    Definition abs (s : single_state) : @Heap (@Node A) := state (ρ s).
+
+    Definition mknode (v : A) (ts : TS) (tk : bool) (nx : Ptr) : @Node A :=
+      pair (pair (pair v ts) tk) nx.
+    Definition mkrec (lv lts lt ln : Addr) : @NodeRec :=
+      pair (pair (pair lv lts) lt) ln.
+
+    Ltac simpl_fields H :=
+      cbn [rec_val rec_ts rec_taken rec_next mkrec node_val node_ts node_taken
+           node_next mknode fst snd] in H.
+    Ltac simpl_fields_goal :=
+      cbn [rec_val rec_ts rec_taken rec_next mkrec node_val node_ts node_taken
+           node_next mknode fst snd].
+
+
+    Definition fields_defined (c : State (li_lts E)) (r : @NodeRec) : Prop :=
+      val_h c (rec_val r) <> None /\ ts_h c (rec_ts r) <> None /\
+      taken_h c (rec_taken r) <> None /\ next_h c (rec_next r) <> None.
+
+    Definition represents (c : State (li_lts E)) (r : @NodeRec) (n : @Node A) : Prop :=
+      val_h c (rec_val r) = Some (node_val n) /\
+      ts_h c (rec_ts r) = Some (node_ts n) /\
+      taken_h c (rec_taken r) = Some (node_taken n) /\
+      next_h c (rec_next r) = Some (node_next n).
+
+    Definition referenced_val (c : State (li_lts E)) (a : Addr) : Prop :=
+      exists l r, rec_h c l = Some r /\ rec_val r = a.
+    Definition referenced_ts (c : State (li_lts E)) (a : Addr) : Prop :=
+      exists l r, rec_h c l = Some r /\ rec_ts r = a.
+    Definition referenced_taken (c : State (li_lts E)) (a : Addr) : Prop :=
+      exists l r, rec_h c l = Some r /\ rec_taken r = a.
+    Definition referenced_next (c : State (li_lts E)) (a : Addr) : Prop :=
+      exists l r, rec_h c l = Some r /\ rec_next r = a.
+
+    (** Facts about the concrete heaps alone.  They hold in every reachable
+        state: the fields of a record are allocated, and distinct records
+        never share a timestamp or a taken cell. *)
+    Definition IConcrete (c : State (li_lts E)) : Prop :=
+      (forall l r, rec_h c l = Some r -> fields_defined c r) /\
+      (forall l1 l2 r1 r2, rec_h c l1 = Some r1 -> rec_h c l2 = Some r2 ->
+        l1 <> l2 -> rec_ts r1 <> rec_ts r2 /\ rec_taken r1 <> rec_taken r2).
+
+    (** The thread [t] is inside [nmsetTS l _] and has not linearized. *)
+    Definition AtSetTS (s : single_state) (t : tid) (l : Addr) : Prop :=
+      exists ts, TMap.find t (π s) = Some (ls_inv (nmsetTS l ts)).
+
+    Definition OtherAtSetTS (s : single_state) (t : tid) (l : Addr) : Prop :=
+      exists t', t <> t' /\ AtSetTS s t' l.
+
+    (** A pending store to a timestamp cell belongs to a [setTS] on the node
+        that owns the cell. *)
+    Definition PendingTSWrite (s : single_state) : Prop :=
+      forall st t' a v, ts_c (σ s) = Pending st t' (owrite a v) ->
+        exists l r, rec_h (σ s) l = Some r /\ rec_ts r = a /\ AtSetTS s t' l.
+
+    (** Two unlinearized [setTS] on the same node: the specification's racy
+        error is reachable, and nothing further is owed. *)
+    Definition Err : assertion := fun s =>
+      exists l t1 t2, t1 <> t2 /\ AtSetTS s t1 l /\ AtSetTS s t2 l.
+
+    (** The abstract heap is represented by the record and field memories. *)
+    Definition Rep (s : single_state) : Prop :=
+      (forall l, abs s l = None <-> rec_h (σ s) l = None) /\
+      (forall l r, rec_h (σ s) l = Some r ->
+        exists n, abs s l = Some n /\ represents (σ s) r n).
+
+    Definition I : assertion := fun s =>
+      (exists h, ρ s = Idle h) /\ IConcrete (σ s) /\ PendingTSWrite s /\
+      (Err s \/ Rep s).
+
+    (** * Thread-local assertions *)
+
+    Definition Defined (l : Addr) : assertion := fun s => rec_h (σ s) l <> None.
+    Definition RecIs (l : Addr) (r : @NodeRec) : assertion :=
+      fun s => rec_h (σ s) l = Some r.
+
+    Definition FreshVal (t : tid) (a : Addr) (v : A) : assertion := fun s =>
+      val_h (σ s) a = Some v /\ val_o (σ s) a = Some t /\ ~ referenced_val (σ s) a.
+    Definition FreshTS (t : tid) (a : Addr) : assertion := fun s =>
+      ts_h (σ s) a = Some TSTop /\ ts_o (σ s) a = Some t /\ ~ referenced_ts (σ s) a.
+    Definition FreshTaken (t : tid) (a : Addr) : assertion := fun s =>
+      taken_h (σ s) a = Some false /\ taken_o (σ s) a = Some t /\
+      ~ referenced_taken (σ s) a.
+    Definition FreshNext (t : tid) (a : Addr) (nx : Ptr) : assertion := fun s =>
+      next_h (σ s) a = Some nx /\ next_o (σ s) a = Some t /\
+      ~ referenced_next (σ s) a.
+
+    Definition AbsTSTop (l : Addr) : assertion :=
+      fun s => exists n, abs s l = Some n /\ node_ts n = TSTop.
+
+    (** [setTS] has read [TSTop]: the abstract timestamp is still [TSTop]
+        (unless the racy error is already reachable), and it stays so while
+        the actor is unlinearized. *)
+    Definition TSTopSeen (t : tid) (l : Addr) (ts : TS) : assertion := fun s =>
+      TMap.find t (π s) = Some (ls_inv (nmsetTS l ts)) /\ (Err s \/ AbsTSTop l s).
+
+    (** * Rely and guarantee *)
+
+    Definition HeapRely (c c' : State (li_lts E)) : Prop :=
+      (forall l r, rec_h c l = Some r -> rec_h c' l = Some r) /\
+      (forall a o, val_h c a <> None -> val_o c a = Some o -> val_o c' a = Some o) /\
+      (forall a o, ts_h c a <> None -> ts_o c a = Some o -> ts_o c' a = Some o) /\
+      (forall a o, taken_h c a <> None -> taken_o c a = Some o ->
+        taken_o c' a = Some o) /\
+      (forall a o, next_h c a <> None -> next_o c a = Some o -> next_o c' a = Some o) /\
+      (forall a v, val_h c a = Some v -> val_h c' a = Some v) /\
+      (forall a v, next_h c a = Some v -> next_h c' a = Some v) /\
+      (forall a v, ts_h c a = Some v -> ~ referenced_ts c a -> ts_h c' a = Some v) /\
+      (forall a v, taken_h c a = Some v -> ~ referenced_taken c a ->
+        taken_h c' a = Some v).
+
+    Definition NewRecOwner (P : option tid -> Prop) (c c' : State (li_lts E)) : Prop :=
+      forall l r, rec_h c l = None -> rec_h c' l = Some r ->
+        P (val_o c' (rec_val r)) /\ P (ts_o c' (rec_ts r)) /\
+        P (taken_o c' (rec_taken r)) /\ P (next_o c' (rec_next r)).
+
+    (** Guarantee of [t]: other threads' linearization tokens are untouched;
+        records are immutable and a new record owns its fields; unreferenced
+        cells never change; the abstract timestamp of a node changes only
+        when no other thread is inside an unlinearized [setTS] on it; and a
+        thread inside a racing [setTS] does not linearize. *)
+    Definition G (t : tid) : rg_relation := fun s s' =>
+      (forall t', t <> t' -> TMap.find t' (π s) = TMap.find t' (π s')) /\
+      HeapRely (σ s) (σ s') /\
+      NewRecOwner (fun o => o = Some t) (σ s) (σ s') /\
+      (forall l n, abs s l = Some n -> exists n', abs s' l = Some n' /\
+        (node_ts n' <> node_ts n -> ~ OtherAtSetTS s t l)) /\
+      (forall l, AtSetTS s t l -> OtherAtSetTS s t l ->
+        TMap.find t (π s) = TMap.find t (π s')).
+
+    Definition R (t : tid) : rg_relation := fun s s' =>
+      TMap.find t (π s) = TMap.find t (π s') /\
+      HeapRely (σ s) (σ s') /\
+      NewRecOwner (fun o => o <> Some t) (σ s) (σ s') /\
+      (forall l n, abs s l = Some n -> exists n', abs s' l = Some n' /\
+        (node_ts n' <> node_ts n -> ~ AtSetTS s t l)) /\
+      (Err s -> Err s').
+
+    Lemma HeapRely_refl c : HeapRely c c.
+    Proof. unfold HeapRely. repeat split; auto. Qed.
+
+    (** * Stability *)
+
+    Lemma I_stable t : Stable (R t) I I.
+    Proof. apply Stable_invariant. Qed.
+
+    Lemma ALin_stable t ls : Stable (R t) I (ALin t ls).
+    Proof.
+      intros s [[pre [Hlin [Hπ _]]] _]. unfold ALin in *. congruence.
+    Qed.
+
+    Lemma Pure_stable t (P : Prop) : Stable (R t) I (⌜P⌝).
+    Proof. apply APureStable. Qed.
+
+    Lemma Err_stable t : Stable (R t) I Err.
+    Proof.
+      intros s [[pre [Herr [_ [_ [_ [_ HR]]]]]] _]. exact (HR Herr).
+    Qed.
+
+    Lemma Defined_stable t l : Stable (R t) I (Defined l).
+    Proof.
+      intros s [[pre [Hdef [_ [[Hrec _] _]]]] _].
+      unfold Defined in *. destruct (rec_h (σ pre) l) as [r|] eqn:Hr;
+        [|contradiction].
+      rewrite (Hrec _ _ Hr). discriminate.
+    Qed.
+
+    Lemma RecIs_stable t l r : Stable (R t) I (RecIs l r).
+    Proof.
+      intros s [[pre [Hr [_ [[Hrec _] _]]]] _]. unfold RecIs in *. auto.
+    Qed.
+
+    Lemma FreshVal_stable t a v : Stable (R t) I (FreshVal t a v).
+    Proof.
+      intros s [[pre [[Hh [Ho Hnr]] [_ [HH [Hnew _]]]]] _].
+      destruct HH as [Hrec [Hown [_ [_ [_ [Hvh _]]]]]].
+      split; [auto|]. split; [eapply Hown; [congruence|exact Ho]|].
+      intros [l [r [Hl Hr]]]. subst a.
+      destruct (rec_h (σ pre) l) as [r0|] eqn:Hr0.
+      - pose proof (Hrec _ _ Hr0) as Hr1. rewrite Hr1 in Hl. injection Hl as ->.
+        apply Hnr. exists l, r. auto.
+      - destruct (Hnew _ _ Hr0 Hl) as [Hnewo _]. apply Hnewo.
+        apply Hown; [congruence|exact Ho].
+    Qed.
+
+    Lemma FreshTS_stable t a : Stable (R t) I (FreshTS t a).
+    Proof.
+      intros s [[pre [[Hh [Ho Hnr]] [_ [HH [Hnew _]]]]] _].
+      destruct HH as [Hrec [_ [Hown [_ [_ [_ [_ [Hth _]]]]]]]].
+      split; [auto|]. split; [eapply Hown; [congruence|exact Ho]|].
+      intros [l [r [Hl Hr]]]. subst a.
+      destruct (rec_h (σ pre) l) as [r0|] eqn:Hr0.
+      - pose proof (Hrec _ _ Hr0) as Hr1. rewrite Hr1 in Hl. injection Hl as ->.
+        apply Hnr. exists l, r. auto.
+      - destruct (Hnew _ _ Hr0 Hl) as [_ [Hnewo _]]. apply Hnewo.
+        apply Hown; [congruence|exact Ho].
+    Qed.
+
+    Lemma FreshTaken_stable t a : Stable (R t) I (FreshTaken t a).
+    Proof.
+      intros s [[pre [[Hh [Ho Hnr]] [_ [HH [Hnew _]]]]] _].
+      destruct HH as [Hrec [_ [_ [Hown [_ [_ [_ [_ Hkh]]]]]]]].
+      split; [auto|]. split; [eapply Hown; [congruence|exact Ho]|].
+      intros [l [r [Hl Hr]]]. subst a.
+      destruct (rec_h (σ pre) l) as [r0|] eqn:Hr0.
+      - pose proof (Hrec _ _ Hr0) as Hr1. rewrite Hr1 in Hl. injection Hl as ->.
+        apply Hnr. exists l, r. auto.
+      - destruct (Hnew _ _ Hr0 Hl) as [_ [_ [Hnewo _]]]. apply Hnewo.
+        apply Hown; [congruence|exact Ho].
+    Qed.
+
+    Lemma FreshNext_stable t a nx : Stable (R t) I (FreshNext t a nx).
+    Proof.
+      intros s [[pre [[Hh [Ho Hnr]] [_ [HH [Hnew _]]]]] _].
+      destruct HH as [Hrec [_ [_ [_ [Hown [_ [Hnh _]]]]]]].
+      split; [auto|]. split; [eapply Hown; [congruence|exact Ho]|].
+      intros [l [r [Hl Hr]]]. subst a.
+      destruct (rec_h (σ pre) l) as [r0|] eqn:Hr0.
+      - pose proof (Hrec _ _ Hr0) as Hr1. rewrite Hr1 in Hl. injection Hl as ->.
+        apply Hnr. exists l, r. auto.
+      - destruct (Hnew _ _ Hr0 Hl) as [_ [_ [_ Hnewo]]]. apply Hnewo.
+        apply Hown; [congruence|exact Ho].
+    Qed.
+
+    Lemma TSTopSeen_stable t l ts : Stable (R t) I (TSTopSeen t l ts).
+    Proof.
+      intros s [[pre [[Hlin Habs] [Hπ [_ [_ [Hts HErr]]]]]] _].
+      split; [congruence|].
+      destruct Habs as [Herr | [n [Hn Htop]]].
+      - left. exact (HErr Herr).
+      - right. destruct (Hts _ _ Hn) as [n' [Hn' Hchange]].
+        exists n'. split; [exact Hn'|].
+        destruct (classic (node_ts n' = node_ts n)) as [Heq|Hneq].
+        + congruence.
+        + exfalso. apply (Hchange Hneq). exists ts. exact Hlin.
+    Qed.
+
+    Create HintDb stableDB.
+    #[local] Hint Resolve I_stable ALin_stable Pure_stable Err_stable
+      Defined_stable RecIs_stable FreshVal_stable FreshTS_stable
+      FreshTaken_stable FreshNext_stable TSTopSeen_stable : stableDB.
+
+    (** * Rely/guarantee side conditions *)
+
+    Lemma source_valid_rg t : forall s s', R t s s' -> I s' ->
+      TMap.find t (π s) = None <-> TMap.find t (π s') = None.
+    Proof. intros s s' [Hπ _] _. rewrite Hπ. tauto. Qed.
+
+    Lemma R_refl t s : R t s s.
+    Proof.
+      split; [reflexivity|]. split; [apply HeapRely_refl|].
+      split; [intros l r H1 H2; congruence|].
+      split; [|auto].
+      intros l n Hn. exists n. split; [exact Hn|]. intros Hc. contradiction.
+    Qed.
+
+    Lemma source_rg_compatible t1 t2 : t1 <> t2 -> forall s s',
+      (G t1 s s' \/ (GINV t1 s s' \/ GRET t1 s s') \/ GId s s') ->
+      R t2 s s'.
+    Proof.
+      intros Hneq s s' [HG | [[Hinv | Hret] | Hid]].
+      - destruct HG as [Hπ [HH [Hnew [Habs Hprot]]]].
+        split; [apply Hπ; exact Hneq|]. split; [exact HH|]. split.
+        + intros l r Hnone Hsome.
+          destruct (Hnew _ _ Hnone Hsome) as [H1 [H2 [H3 H4]]].
+          rewrite H1, H2, H3, H4.
+          repeat split; intros Heq; injection Heq; intros; congruence.
+        + split.
+          * intros l n Hn. destruct (Habs _ _ Hn) as [n' [Hn' Hch]].
+            exists n'. split; [exact Hn'|].
+            intros Hts Hat. apply (Hch Hts). exists t2. split; auto.
+          * intros [l [ta [tb [Hab [Ha Hb]]]]]. exists l, ta, tb.
+            split; [exact Hab|].
+            assert (Hkeep : forall tx ty, tx <> ty ->
+              AtSetTS s tx l -> AtSetTS s ty l -> AtSetTS s' tx l).
+            { intros tx ty Hxy [ts Hx] Hy. exists ts.
+              destruct (Pos.eq_dec t1 tx) as [->|Hne].
+              - rewrite <- (Hprot l); [exact Hx|exists ts; exact Hx|].
+                exists ty. split; auto.
+              - rewrite <- Hπ; auto. }
+            split; [eapply Hkeep; eauto|eapply Hkeep; eauto].
+      - destruct Hinv as [f [Hσ [Hρ [Hnone Hπ]]]].
+        unfold R, abs. rewrite <- Hσ, <- Hρ, Hπ.
+        split; [rewrite TMap.gso; auto|].
+        split; [apply HeapRely_refl|].
+        split; [intros l r H1 H2; congruence|].
+        split; [intros l n Hn; exists n; split; [exact Hn|intros Hc; contradiction]|].
+        intros [l [ta [tb [Hab [[tsa Ha] [tsb Hb]]]]]].
+        exists l, ta, tb. split; [exact Hab|].
+        split; [exists tsa|exists tsb]; rewrite Hπ, TMap.gso; auto; congruence.
+      - destruct Hret as [f [ret [Hσ [Hρ [Hsome Hπ]]]]].
+        unfold R, abs. rewrite <- Hσ, <- Hρ, Hπ.
+        split; [rewrite TMap.gro; auto|].
+        split; [apply HeapRely_refl|].
+        split; [intros l r H1 H2; congruence|].
+        split; [intros l n Hn; exists n; split; [exact Hn|intros Hc; contradiction]|].
+        intros [l [ta [tb [Hab [[tsa Ha] [tsb Hb]]]]]].
+        exists l, ta, tb. split; [exact Hab|].
+        split; [exists tsa|exists tsb]; rewrite Hπ, TMap.gro; auto; congruence.
+      - unfold GId in Hid. subst. apply R_refl.
+    Qed.
+
+    (** * Reaching the specification's errors *)
+
+    Lemma Err_APError : ⊨ I //\\ Err ==>> APError.
+    Proof.
+      intros s [[[h Hρ] _] [l [t1 [t2 [Hneq [[ts1 H1] [ts2 H2]]]]]]].
+      unfold APError. rewrite Hρ.
+      destruct (h l) eqn:Hl.
+      - eapply rt_trans.
+        + apply rt_step. apply (ps_inv t1 (nmsetTS l ts1)); [|exact H1].
+          apply step_inv. eapply step_setTS_inv; [reflexivity|].
+          rewrite Hl. discriminate.
+        + apply rt_step. eapply (ps_error t2 (nmsetTS l ts2)).
+          * eapply error_setTS_racy; [| |reflexivity]; [congruence|reflexivity].
+          * rewrite TMap.gso; [exact H2|congruence].
+      - apply rt_step. eapply (ps_error t1 (nmsetTS l ts1)); [|exact H1].
+        eapply error_setTS_undefined; [reflexivity|exact Hl].
+    Qed.
+
+    Lemma undefined_APError t (f : Sig.op (li_sig F)) l s :
+      I s -> TMap.find t (π s) = Some (ls_inv f) -> abs s l = None ->
+      (forall h, h l = None ->
+        ErrorNodeMem {| te_tid := t; te_ev := InvEv f |} (Idle h)) ->
+      APError s.
+    Proof.
+      intros [[h Hρ] _] Hlin Habs Herr. unfold APError. rewrite Hρ.
+      unfold abs in Habs. rewrite Hρ in Habs. simpl in Habs.
+      apply rt_step. eapply (ps_error t f); [|exact Hlin].
+      apply Herr. exact Habs.
+    Qed.
+
+    (** Every method except allocation starts by reading the record cell.
+        Either the node is allocated, or the specification is in error. *)
+    Lemma defined_or_error t (f : Sig.op (li_sig F)) l :
+      (forall h, h l = None ->
+        ErrorNodeMem {| te_tid := t; te_ev := InvEv f |} (Idle h)) ->
+      ⊨ I //\\ ALin t (ls_inv f) ==>>
+        (I //\\ ALin t (ls_inv f) //\\ Defined l) \\// APError.
+    Proof.
+      intros Herr s [HI Hlin]. pose proof HI as [Hρ [Hc [Hp Hor]]].
+      destruct Hor as [HErr | [Hnone Hsome]].
+      - right. apply Err_APError. split; assumption.
+      - destruct (abs s l) as [n|] eqn:Hl.
+        + left. split; [exact HI|]. split; [exact Hlin|].
+          unfold Defined. intros Hrec. apply Hnone in Hrec.
+          rewrite Hl in Hrec. discriminate.
+        + right. eapply undefined_APError; eauto.
+    Qed.
+
+    (** * Underlay steps never error *)
+
+    Lemma alloc_val_no_error t v (P : assertion) :
+      ⊨ P ==>> ANoError {| te_tid := t; te_ev := InvEv (in_val (omalloc v)) |}.
+    Proof.
+      intros s _ Herr. apply (error_val t (InvEv (omalloc v))) in Herr.
+      eapply omem_alloc_no_error; exact Herr.
+    Qed.
+
+    Lemma alloc_ts_no_error t v (P : assertion) :
+      ⊨ P ==>> ANoError {| te_tid := t; te_ev := InvEv (in_ts (omalloc v)) |}.
+    Proof.
+      intros s _ Herr. apply (error_ts t (InvEv (omalloc v))) in Herr.
+      eapply omem_alloc_no_error; exact Herr.
+    Qed.
+
+    Lemma alloc_next_no_error t v (P : assertion) :
+      ⊨ P ==>> ANoError {| te_tid := t; te_ev := InvEv (in_next (omalloc v)) |}.
+    Proof.
+      intros s _ Herr. apply (error_next t (InvEv (omalloc v))) in Herr.
+      eapply omem_alloc_no_error; exact Herr.
+    Qed.
+
+    Lemma alloc_taken_no_error t v (P : assertion) :
+      ⊨ P ==>> ANoError {| te_tid := t; te_ev := InvEv (in_taken (omalloc v)) |}.
+    Proof.
+      intros s _ Herr. apply (error_taken t (InvEv (omalloc v))) in Herr.
+      eapply omem_alloc_no_error; exact Herr.
+    Qed.
+
+    Lemma alloc_rec_no_error t v (P : assertion) :
+      ⊨ P ==>> ANoError {| te_tid := t; te_ev := InvEv (in_rec (omalloc v)) |}.
+    Proof.
+      intros s _ Herr. apply (error_rec t (InvEv (omalloc v))) in Herr.
+      eapply omem_alloc_no_error; exact Herr.
+    Qed.
+
+    Lemma read_rec_no_error t l (P : assertion) :
+      (⊨ P ==>> Defined l) ->
+      ⊨ P ==>> ANoError {| te_tid := t; te_ev := InvEv (in_rec (oread l)) |}.
+    Proof.
+      intros HP s HPs Herr. pose proof (HP s HPs) as Hdef. apply (error_rec t (InvEv (oread l))) in Herr.
+      eapply omem_read_no_error; [exact Hdef|exact Herr].
+    Qed.
+
+    Lemma I_fields_defined l r s :
+      I s -> RecIs l r s -> fields_defined (σ s) r.
+    Proof. intros [_ [[Hf _] _]] Hr. apply (Hf _ _ Hr). Qed.
+
+    Lemma read_val_no_error t l r (P : assertion) :
+      (⊨ P ==>> I //\\ RecIs l r) ->
+      ⊨ P ==>> ANoError {| te_tid := t; te_ev := InvEv (in_val (oread (rec_val r))) |}.
+    Proof.
+      intros HP s HPs Herr. destruct (HP s HPs) as [HI Hr]. apply (error_val t (InvEv (oread (rec_val r)))) in Herr.
+      destruct (I_fields_defined _ _ _ HI Hr) as [Hdef _].
+      eapply omem_read_no_error; [exact Hdef|exact Herr].
+    Qed.
+
+    Lemma read_ts_no_error t l r (P : assertion) :
+      (⊨ P ==>> I //\\ RecIs l r) ->
+      ⊨ P ==>> ANoError {| te_tid := t; te_ev := InvEv (in_ts (oread (rec_ts r))) |}.
+    Proof.
+      intros HP s HPs Herr. destruct (HP s HPs) as [HI Hr]. apply (error_ts t (InvEv (oread (rec_ts r)))) in Herr.
+      destruct (I_fields_defined _ _ _ HI Hr) as [_ [Hdef _]].
+      eapply omem_read_no_error; [exact Hdef|exact Herr].
+    Qed.
+
+    Lemma read_taken_no_error t l r (P : assertion) :
+      (⊨ P ==>> I //\\ RecIs l r) ->
+      ⊨ P ==>> ANoError {| te_tid := t; te_ev := InvEv (in_taken (oread (rec_taken r))) |}.
+    Proof.
+      intros HP s HPs Herr. destruct (HP s HPs) as [HI Hr].
+      apply (error_taken t (InvEv (oread (rec_taken r)))) in Herr.
+      destruct (I_fields_defined _ _ _ HI Hr) as [_ [_ [Hdef _]]].
+      eapply omem_read_no_error; [exact Hdef|exact Herr].
+    Qed.
+
+    Lemma read_next_no_error t l r (P : assertion) :
+      (⊨ P ==>> I //\\ RecIs l r) ->
+      ⊨ P ==>> ANoError {| te_tid := t; te_ev := InvEv (in_next (oread (rec_next r))) |}.
+    Proof.
+      intros HP s HPs Herr. destruct (HP s HPs) as [HI Hr].
+      apply (error_next t (InvEv (oread (rec_next r)))) in Herr.
+      destruct (I_fields_defined _ _ _ HI Hr) as [_ [_ [_ Hdef]]].
+      eapply omem_read_no_error; [exact Hdef|exact Herr].
+    Qed.
+
+    Lemma cas_taken_no_error t l r v w (P : assertion) :
+      (⊨ P ==>> I //\\ RecIs l r) ->
+      ⊨ P ==>> ANoError {| te_tid := t; te_ev := InvEv (in_taken (ocas (rec_taken r) v w)) |}.
+    Proof.
+      intros HP s HPs Herr. destruct (HP s HPs) as [HI Hr].
+      apply (error_taken t (InvEv (ocas (rec_taken r) v w))) in Herr.
+      destruct (I_fields_defined _ _ _ HI Hr) as [_ [_ [Hdef _]]].
+      eapply omem_cas_no_error; [exact Hdef|exact Herr].
+    Qed.
+
+    (** No other thread has a pending store to the timestamp cell [a]. *)
+    Definition NoOtherTSWrite (t : tid) (a : Addr) : assertion := fun s =>
+      forall st t' v, ts_c (σ s) = Pending st t' (owrite a v) -> t = t'.
+
+    (** Before storing the timestamp: either the store is race free, or the
+        other writer is inside a [setTS] on the same node and the
+        specification's racy error is reachable. *)
+    Lemma ts_write_race_or_error t l r ts :
+      ⊨ I //\\ TSTopSeen t l ts //\\ RecIs l r ==>>
+        (I //\\ TSTopSeen t l ts //\\ RecIs l r //\\ NoOtherTSWrite t (rec_ts r))
+        \\// APError.
+    Proof.
+      intros s [HI [Hseen Hr]].
+      destruct (classic (exists st t' v,
+        ts_c (σ s) = Pending st t' (owrite (rec_ts r) v) /\ t <> t'))
+        as [[st [t' [v [Hpend Hneq]]]] | Hno].
+      - right. apply Err_APError. split; [exact HI|].
+        destruct HI as [_ [[_ Hinj] [Hp _]]].
+        destruct (Hp _ _ _ _ Hpend) as [l' [r' [Hr' [Hts' Hat']]]].
+        destruct (Nat.eq_dec l l') as [<-|Hll].
+        + exists l, t, t'. split; [exact Hneq|]. split; [|exact Hat'].
+          exists ts. apply Hseen.
+        + exfalso. destruct (Hinj _ _ _ _ Hr Hr' Hll) as [Hne _]. congruence.
+      - left. split; [exact HI|]. split; [exact Hseen|]. split; [exact Hr|].
+        intros st t' v Hpend. destruct (Pos.eq_dec t t') as [Heq|Hneq]; [exact Heq|].
+        exfalso. apply Hno. exists st, t', v. auto.
+    Qed.
+
+    Lemma write_ts_no_error t l r ts :
+      ⊨ I //\\ TSTopSeen t l ts //\\ RecIs l r //\\ NoOtherTSWrite t (rec_ts r) ==>>
+        ANoError {| te_tid := t; te_ev := InvEv (in_ts (owrite (rec_ts r) ts)) |}.
+    Proof.
+      intros s [HI [_ [Hr Hno]]] Herr.
+      apply (error_ts t (InvEv (owrite (rec_ts r) ts))) in Herr.
+      destruct (I_fields_defined _ _ _ HI Hr) as [_ [Hdef _]].
+      eapply omem_write_no_error; [exact Hdef| |exact Herr].
+      intros st t' v' Hpend. apply (Hno st t' v'). exact Hpend.
+    Qed.
+
+    (** * Building blocks for possibility updates *)
+
+    Definition st (c : State (li_lts E)) (a : State (li_lts F))
+        (p : tmap (@LinState (li_sig F))) : single_state :=
+      @SinglePossState.Build_ProofStateSingle _ _ (li_lts E) (li_lts F) c a p.
+
+    Ltac simpl_abs := unfold abs; cbn [st SinglePossState.ρ state].
+
+    (** Facts about the linearization map alone. *)
+    Definition AtSetTSPi (p : tmap (@LinState (li_sig F))) (t : tid) (l : Addr) :=
+      exists ts, TMap.find t p = Some (ls_inv (nmsetTS l ts)).
+
+    Lemma AtSetTS_pi s t l : AtSetTS s t l <-> AtSetTSPi (π s) t l.
+    Proof. reflexivity. Qed.
+
+    (** Two facts about the same entry.  Stated with [eq_trans] because the
+        implicit signature of the entries differs up to unfolding
+        ([@ENodeMem A] versus [li_sig F]), which defeats [rewrite]. *)
+    Lemma AtSetTS_self t (f : Sig.op (li_sig F)) (p : tmap (@LinState (li_sig F))) l :
+      TMap.find t p = Some (ls_inv f) -> AtSetTSPi p t l ->
+      exists ts, f = nmsetTS l ts.
+    Proof.
+      intros Hlin [ts Hts]. exists ts.
+      pose proof (eq_trans (eq_sym Hlin) Hts) as Heq. injection Heq as Heq. exact Heq.
+    Qed.
+
+    Lemma AtSetTS_self_setTS t l ts (p : tmap (@LinState (li_sig F))) l0 :
+      TMap.find t p = Some (ls_inv (nmsetTS l ts)) -> AtSetTSPi p t l0 -> l0 = l.
+    Proof.
+      intros Hlin Hat. destruct (AtSetTS_self _ _ _ _ Hlin Hat) as [ts' Heq].
+      injection Heq as Heq _. symmetry. exact Heq.
+    Qed.
+
+    Definition lin_π t (f : Sig.op (li_sig F)) (ret : Sig.ar f)
+        (p : tmap (@LinState (li_sig F))) :=
+      TMap.add t (ls_linr f ret) (TMap.add t (ls_lini f) p).
+
+    Lemma lin_π_self t (f : Sig.op (li_sig F)) ret (p : tmap (@LinState (li_sig F))) :
+      TMap.find t (lin_π t f ret p) = Some (ls_linr f ret).
+    Proof. unfold lin_π. apply TMap.gss. Qed.
+
+    Lemma lin_π_other t t' (f : Sig.op (li_sig F)) ret (p : tmap (@LinState (li_sig F))) :
+      t <> t' -> TMap.find t' (lin_π t f ret p) = TMap.find t' p.
+    Proof. intros Hne. unfold lin_π. rewrite !TMap.gso; auto. Qed.
+
+    (** Linearizing an entire abstract operation at once. *)
+    Lemma lin_steps t (f : Sig.op (li_sig F)) (ret : Sig.ar f) h h'
+        (p : tmap (@LinState (li_sig F))) :
+      TMap.find t p = Some (ls_inv f) ->
+      StepNodeMem {| te_tid := t; te_ev := InvEv f |} h h ->
+      StepNodeMem {| te_tid := t; te_ev := ResEv f ret |} h h' ->
+      @poss_steps _ (li_lts F) (@PossOk _ (li_lts F) (Idle h) p)
+        (@PossOk _ (li_lts F) (Idle h') (lin_π t f ret p)).
+    Proof.
+      intros Hlin Hinv Hres. eapply rt_trans.
+      - apply rt_step. apply (ps_inv t f); [|exact Hlin].
+        apply step_inv. exact Hinv.
+      - apply rt_step. apply (ps_ret t f ret).
+        + apply step_res. exact Hres.
+        + apply TMap.gss.
+    Qed.
+
+    (** Every other thread's entry, and every [AtSetTS] fact, survives the
+        actor's linearization of an operation that is not [nmsetTS]. *)
+    Lemma AtSetTS_lin t (f : Sig.op (li_sig F)) ret (p : tmap (@LinState (li_sig F))) :
+      TMap.find t p = Some (ls_inv f) ->
+      (forall l ts, f <> nmsetTS l ts) ->
+      forall t' l, AtSetTSPi p t' l -> AtSetTSPi (lin_π t f ret p) t' l.
+    Proof.
+      intros Hlin Hf t' l Hat.
+      destruct (Pos.eq_dec t t') as [<-|Hne].
+      - exfalso. destruct (AtSetTS_self _ _ _ _ Hlin Hat) as [ts Heq]. eapply Hf; exact Heq.
+      - destruct Hat as [ts Hts]. exists ts. rewrite lin_π_other; auto.
+    Qed.
+
+    (** Heap facts. *)
+    Lemma heap_update_defined {V} (h : @Heap V) l v a :
+      h a <> None -> heap_update l v h a <> None.
+    Proof.
+      intros Hdef. unfold heap_update. destruct (Nat.eqb l a); [discriminate|exact Hdef].
+    Qed.
+
+    Lemma heap_update_fresh {V} (h : @Heap V) l v a x :
+      h l = None -> h a = Some x -> heap_update l v h a = Some x.
+    Proof.
+      intros Hl Ha. rewrite HeapUpdateOther; [exact Ha|]. congruence.
+    Qed.
+
+    Lemma heap_update_none_iff {V} (h : @Heap V) l v a n :
+      h l = Some n -> (heap_update l v h a = None <-> h a = None).
+    Proof.
+      intros Hl. unfold heap_update. destruct (Nat.eqb l a) eqn:Heq.
+      - apply Nat.eqb_eq in Heq. subst. rewrite Hl. split; discriminate.
+      - tauto.
+    Qed.
+
+    Lemma heap_update_same {V} (h : @Heap V) l n :
+      h l = Some n -> heap_update l n h = h.
+    Proof.
+      intros Hl. apply functional_extensionality. intros a.
+      unfold heap_update. destruct (Nat.eqb l a) eqn:Heq; [|reflexivity].
+      apply Nat.eqb_eq in Heq. subst. auto.
+    Qed.
+
+    Lemma node_eta (n : @Node A) :
+      n = mknode (node_val n) (node_ts n) (node_taken n) (node_next n).
+    Proof. destruct n as [[[v ts] tk] nx]. reflexivity. Qed.
+
+    (** Invariant pieces that only depend on unchanged heaps. *)
+    Definition same_heaps (c c' : State (li_lts E)) : Prop :=
+      rec_h c' = rec_h c /\ val_h c' = val_h c /\ val_o c' = val_o c /\
+      ts_h c' = ts_h c /\ ts_o c' = ts_o c /\ taken_h c' = taken_h c /\
+      taken_o c' = taken_o c /\ next_h c' = next_h c /\ next_o c' = next_o c.
+
+    Lemma IConcrete_same c c' :
+      same_heaps c c' -> IConcrete c -> IConcrete c'.
+    Proof.
+      intros (Hr & Hv & _ & Ht & _ & Hk & _ & Hn & _) [Hf Hinj].
+      unfold IConcrete, fields_defined. rewrite Hr, Hv, Ht, Hk, Hn. auto.
+    Qed.
+
+    Lemma Rep_same c c' a p p' :
+      same_heaps c c' -> Rep (st c a p) -> Rep (st c' a p').
+    Proof.
+      intros (Hr & Hv & _ & Ht & _ & Hk & _ & Hn & _) [H1 H2].
+      unfold Rep, represents, abs in *. simpl in *. rewrite Hr, Hv, Ht, Hk, Hn. auto.
+    Qed.
+
+    Lemma HeapRely_same c c' : same_heaps c c' -> HeapRely c c'.
+    Proof.
+      intros (Hr & Hv & Hvo & Ht & Hto & Hk & Hko & Hn & Hno).
+      unfold HeapRely. rewrite Hr, Hv, Hvo, Ht, Hto, Hk, Hko, Hn, Hno.
+      repeat split; auto.
+    Qed.
+
+    (** The timestamp control of [c'] carries no pending store that [c] did
+        not already carry. *)
+    Definition no_new_ts_write (c c' : State (li_lts E)) : Prop :=
+      forall st0 t' x v, ts_c c' = Pending st0 t' (owrite x v) ->
+        ts_c c = Pending st0 t' (owrite x v).
+
+    Lemma no_new_ts_write_eq c c' : ts_c c' = ts_c c -> no_new_ts_write c c'.
+    Proof. intros Heq st0 t' x v H. rewrite <- Heq. exact H. Qed.
+
+    Lemma no_new_ts_write_idle c c' s : ts_c c' = Idle s -> no_new_ts_write c c'.
+    Proof. intros Heq st0 t' x v H. rewrite Heq in H. discriminate. Qed.
+
+    Lemma PendingTSWrite_grow c c' a a' p p' :
+      no_new_ts_write c c' ->
+      (forall l r, rec_h c l = Some r -> rec_h c' l = Some r) ->
+      (forall t' l, AtSetTSPi p t' l -> AtSetTSPi p' t' l) ->
+      PendingTSWrite (st c a p) -> PendingTSWrite (st c' a' p').
+    Proof.
+      intros Hts Hr Hpi Hp st0 t' x v Hpend. simpl in Hpend. apply Hts in Hpend.
+      destruct (Hp _ _ _ _ Hpend) as [l [r [Hl [Hx Hat]]]].
+      exists l, r. simpl. split; [apply Hr; exact Hl|]. split; [exact Hx|].
+      apply Hpi. exact Hat.
+    Qed.
+
+    Lemma PendingTSWrite_same c c' a a' p p' :
+      no_new_ts_write c c' -> rec_h c' = rec_h c ->
+      (forall t' l, AtSetTSPi p t' l -> AtSetTSPi p' t' l) ->
+      PendingTSWrite (st c a p) -> PendingTSWrite (st c' a' p').
+    Proof.
+      intros Hts Hr. apply PendingTSWrite_grow; [exact Hts|].
+      intros l r Hl. rewrite Hr. exact Hl.
+    Qed.
+
+    Lemma Err_pi c c' a a' p p' :
+      (forall t' l, AtSetTSPi p t' l -> AtSetTSPi p' t' l) ->
+      Err (st c a p) -> Err (st c' a' p').
+    Proof.
+      intros Hpi [l [t1 [t2 [Hne [H1 H2]]]]]. exists l, t1, t2.
+      split; [exact Hne|]. split; apply Hpi; assumption.
+    Qed.
+
+    Lemma I_same c c' a p p' :
+      same_heaps c c' -> no_new_ts_write c c' ->
+      (forall t' l, AtSetTSPi p t' l -> AtSetTSPi p' t' l) ->
+      I (st c a p) -> I (st c' a p').
+    Proof.
+      intros Hsame Hts Hpi [Hρ [Hc [Hp Hor]]].
+      split; [exact Hρ|]. split; [eapply IConcrete_same; eauto|].
+      split; [eapply PendingTSWrite_same; eauto; apply Hsame|].
+      destruct Hor as [Herr|Hrep].
+      - left. eapply Err_pi; eauto.
+      - right. eapply Rep_same; eauto.
+    Qed.
+
+    (** A guarantee step that changes no heap and no abstract state. *)
+    Lemma G_same t c c' a p p' :
+      same_heaps c c' ->
+      (forall t', t <> t' -> TMap.find t' p = TMap.find t' p') ->
+      (forall l, AtSetTSPi p t l -> (exists t', t <> t' /\ AtSetTSPi p t' l) ->
+        TMap.find t p = TMap.find t p') ->
+      G t (st c a p) (st c' a p').
+    Proof.
+      intros Hsame Hπ Hprot. split; [exact Hπ|].
+      split; [apply HeapRely_same; exact Hsame|].
+      split; [intros l r H1 H2; simpl in H1, H2; destruct Hsame as [Hr _];
+              rewrite Hr in H2; congruence|].
+      split.
+      - intros l n Hn. exists n. split; [exact Hn|]. intros Hc. contradiction.
+      - exact Hprot.
+    Qed.
+
+    Lemma same_heaps_control c c' :
+      state (rec_c c') = state (rec_c c) -> state (val_c c') = state (val_c c) ->
+      state (ts_c c') = state (ts_c c) -> state (next_c c') = state (next_c c) ->
+      state (taken_c c') = state (taken_c c) ->
+      same_heaps c c'.
+    Proof.
+      intros H1 H2 H3 H4 H5. unfold same_heaps, rec_h, val_h, val_o, ts_h, ts_o,
+        taken_h, taken_o, next_h, next_o.
+      rewrite H1, H2, H3, H4, H5. repeat split.
+    Qed.
+
+    (** Lifting the error escape to the set logic. *)
+    Lemma lift_perror (P P' : assertion) :
+      (⊨ P ==>> P' \\// APError) ->
+      ⊨ lift_assert P ==>> lift_assert P' \\// AssertionsSet.APError.
+    Proof.
+      intros Himpl s [x [Hview HP]].
+      destruct (Himpl x HP) as [HP'|Herr].
+      - left. exists x. auto.
+      - right. eapply AssertionsSet.APErrorSome.
+        + apply singleton_view_member. exact Hview.
+        + exact Herr.
+    Qed.
+
+    Lemma done_or_err (P : assertion) :
+      ⊨ P \\// (I //\\ Err) ==>> P \\// APError.
+    Proof.
+      intros s [HP | HErr]; [left; exact HP|right; apply Err_APError; exact HErr].
+    Qed.
+
+    Lemma disj_I (P : assertion) :
+      (⊨ P ==>> I) -> ⊨ P \\// (I //\\ Err) ==>> I.
+    Proof. intros HP s [H | [HI _]]; [apply HP; exact H|exact HI]. Qed.
+
+    (** * Method-level assertions *)
+
+    Definition Active t (f : Sig.op (li_sig F)) : assertion :=
+      I //\\ ALin t (ls_inv f).
+    Definition Done t (f : Sig.op (li_sig F)) (ret : Sig.ar f) : assertion :=
+      I //\\ ALin t (ls_linr f ret).
+    Definition DoneOrErr t (f : Sig.op (li_sig F)) (ret : Sig.ar f) : assertion :=
+      Done t f ret \\// (I //\\ Err).
+
+    Lemma Active_I t f : ⊨ Active t f ==>> I.
+    Proof. intros s [HI _]. exact HI. Qed.
+    Lemma Done_I t f ret : ⊨ Done t f ret ==>> I.
+    Proof. intros s [HI _]. exact HI. Qed.
+    Lemma DoneOrErr_I t f ret : ⊨ DoneOrErr t f ret ==>> I.
+    Proof. apply disj_I. apply Done_I. Qed.
+    Lemma Active_stable t f : Stable (R t) I (Active t f).
+    Proof. apply ConjStable; auto with stableDB. Qed.
+    Lemma Done_stable t f ret : Stable (R t) I (Done t f ret).
+    Proof. apply ConjStable; auto with stableDB. Qed.
+    Lemma DoneOrErr_stable t f ret : Stable (R t) I (DoneOrErr t f ret).
+    Proof.
+      apply DisjStable; [apply Done_stable|apply ConjStable; auto with stableDB].
+    Qed.
+    #[local] Hint Resolve Active_stable Done_stable DoneOrErr_stable : stableDB.
+
+    Lemma DoneOrErr_perror t f ret :
+      ⊨ lift_assert (DoneOrErr t f ret) ==>>
+        lift_assert (Done t f ret) \\// AssertionsSet.APError.
+    Proof. apply lift_perror. apply done_or_err. Qed.
+
+    (** Heaps only gain cells; records never change. *)
+    Definition heaps_grow (c c' : State (li_lts E)) : Prop :=
+      rec_h c' = rec_h c /\
+      (forall a v, val_h c a = Some v -> val_h c' a = Some v) /\
+      (forall a o, val_h c a <> None -> val_o c a = Some o -> val_o c' a = Some o) /\
+      (forall a v, ts_h c a = Some v -> ts_h c' a = Some v) /\
+      (forall a o, ts_h c a <> None -> ts_o c a = Some o -> ts_o c' a = Some o) /\
+      (forall a v, taken_h c a = Some v -> taken_h c' a = Some v) /\
+      (forall a o, taken_h c a <> None -> taken_o c a = Some o ->
+        taken_o c' a = Some o) /\
+      (forall a v, next_h c a = Some v -> next_h c' a = Some v) /\
+      (forall a o, next_h c a <> None -> next_o c a = Some o -> next_o c' a = Some o).
+
+    Lemma same_heaps_grow c c' : same_heaps c c' -> heaps_grow c c'.
+    Proof.
+      intros (Hr & Hv & Hvo & Ht & Hto & Hk & Hko & Hn & Hno).
+      unfold heaps_grow. rewrite Hr, Hv, Hvo, Ht, Hto, Hk, Hko, Hn, Hno.
+      repeat split; auto.
+    Qed.
+
+    (** Assertions that do not look at the control components and survive
+        allocation. *)
+    Definition CI (P : assertion) : Prop :=
+      forall c c' a p, heaps_grow c c' -> P (st c a p) -> P (st c' a p).
+
+    Lemma ALin_ci t ls : CI (ALin t ls).
+    Proof. intros c c' a p _ H. exact H. Qed.
+    Lemma Err_ci : CI Err.
+    Proof. intros c c' a p _ H. exact H. Qed.
+    Lemma Defined_ci l : CI (Defined l).
+    Proof. intros c c' a p [Hr _] H. unfold Defined in *. simpl in *. rewrite Hr. exact H. Qed.
+    Lemma RecIs_ci l r : CI (RecIs l r).
+    Proof. intros c c' a p [Hr _] H. unfold RecIs in *. simpl in *. rewrite Hr. exact H. Qed.
+    Lemma FreshVal_ci t x v : CI (FreshVal t x v).
+    Proof.
+      intros c c' a p (Hr & Hv & Hvo & _) [H1 [H2 H3]]. unfold FreshVal, referenced_val in *.
+      simpl in *. rewrite Hr. split; [apply Hv; exact H1|].
+      split; [apply Hvo; [rewrite H1; discriminate|exact H2]|exact H3].
+    Qed.
+    Lemma FreshTS_ci t x : CI (FreshTS t x).
+    Proof.
+      intros c c' a p (Hr & _ & _ & Ht & Hto & _) [H1 [H2 H3]].
+      unfold FreshTS, referenced_ts in *. simpl in *. rewrite Hr.
+      split; [apply Ht; exact H1|].
+      split; [apply Hto; [rewrite H1; discriminate|exact H2]|exact H3].
+    Qed.
+    Lemma FreshTaken_ci t x : CI (FreshTaken t x).
+    Proof.
+      intros c c' a p (Hr & _ & _ & _ & _ & Hk & Hko & _) [H1 [H2 H3]].
+      unfold FreshTaken, referenced_taken in *. simpl in *. rewrite Hr.
+      split; [apply Hk; exact H1|].
+      split; [apply Hko; [rewrite H1; discriminate|exact H2]|exact H3].
+    Qed.
+    Lemma FreshNext_ci t x nx : CI (FreshNext t x nx).
+    Proof.
+      intros c c' a p (Hr & _ & _ & _ & _ & _ & _ & Hn & Hno) [H1 [H2 H3]].
+      unfold FreshNext, referenced_next in *. simpl in *. rewrite Hr.
+      split; [apply Hn; exact H1|].
+      split; [apply Hno; [rewrite H1; discriminate|exact H2]|exact H3].
+    Qed.
+    Lemma TSTopSeen_ci t l ts : CI (TSTopSeen t l ts).
+    Proof. intros c c' a p _ H. exact H. Qed.
+    Lemma Conj_ci (P Q : assertion) : CI P -> CI Q -> CI (P //\\ Q).
+    Proof. intros HP HQ c c' a p Hs [H1 H2]. split; [eapply HP|eapply HQ]; eauto. Qed.
+    Lemma Disj_ci (P Q : assertion) : CI P -> CI Q -> CI (P \\// Q).
+    Proof.
+      intros HP HQ c c' a p Hs [H1 | H2]; [left; eapply HP|right; eapply HQ]; eauto.
+    Qed.
+
+    Create HintDb ciDB.
+    #[local] Hint Resolve ALin_ci Err_ci Defined_ci RecIs_ci FreshVal_ci FreshTS_ci
+      FreshTaken_ci FreshNext_ci TSTopSeen_ci Conj_ci Disj_ci : ciDB.
+
+    (** * Generic possibility updates *)
+
+    (** An invocation on any component memory other than a timestamp store
+        changes only the control state. *)
+    Lemma inv_update t (m : Sig.op (li_sig E)) (P : assertion) :
+      CI P ->
+      (forall x v, m <> in_ts (owrite x v)) ->
+      PUpdate (G t) {| te_tid := t; te_ev := InvEv m |} (I //\\ P) (I //\\ P).
+    Proof.
+      intros HP Hnw σ1 ρ1 π1 [HI Hpre] σ2 Hstep.
+      exists ρ1, π1. split; [apply rt_refl|].
+      assert (Hfacts : same_heaps σ1 σ2 /\
+        (forall st0 t' x v, ts_c σ2 = Pending st0 t' (owrite x v) ->
+          ts_c σ1 = Pending st0 t' (owrite x v))).
+      { destruct m as [[[[m0|m0]|m0]|m0]|m0].
+        - apply (step_rec t (InvEv m0)) in Hstep.
+          destruct Hstep as [Hs [H1 [H2 [H3 H4]]]].
+          destruct (omem_inv_shape _ _ _ _ Hs) as [s [Hc Hc']].
+          split; [|rewrite H2; auto].
+          apply same_heaps_control; [rewrite Hc, Hc'|rewrite H1|rewrite H2|rewrite H3|rewrite H4];
+            reflexivity.
+        - apply (step_val t (InvEv m0)) in Hstep.
+          destruct Hstep as [Hs [H1 [H2 [H3 H4]]]].
+          destruct (omem_inv_shape _ _ _ _ Hs) as [s [Hc Hc']].
+          split; [|rewrite H2; auto].
+          apply same_heaps_control; [rewrite H1|rewrite Hc, Hc'|rewrite H2|rewrite H3|rewrite H4];
+            reflexivity.
+        - apply (step_ts t (InvEv m0)) in Hstep.
+          destruct Hstep as [Hs [H1 [H2 [H3 H4]]]].
+          destruct (omem_inv_shape _ _ _ _ Hs) as [s [Hc Hc']].
+          split.
+          + apply same_heaps_control; [rewrite H1|rewrite H2|rewrite Hc, Hc'|rewrite H3|rewrite H4];
+              reflexivity.
+          + intros st0 t' x v Heq. rewrite Hc' in Heq. injection Heq as _ _ Hm.
+            exfalso. apply (Hnw x v). rewrite Hm. reflexivity.
+        - apply (step_next t (InvEv m0)) in Hstep.
+          destruct Hstep as [Hs [H1 [H2 [H3 H4]]]].
+          destruct (omem_inv_shape _ _ _ _ Hs) as [s [Hc Hc']].
+          split; [|rewrite H3; auto].
+          apply same_heaps_control; [rewrite H1|rewrite H2|rewrite H3|rewrite Hc, Hc'|rewrite H4];
+            reflexivity.
+        - apply (step_taken t (InvEv m0)) in Hstep.
+          destruct Hstep as [Hs [H1 [H2 [H3 H4]]]].
+          destruct (omem_inv_shape _ _ _ _ Hs) as [s [Hc Hc']].
+          split; [|rewrite H3; auto].
+          apply same_heaps_control; [rewrite H1|rewrite H2|rewrite H3|rewrite H4|rewrite Hc, Hc'];
+            reflexivity. }
+      destruct Hfacts as [Hsame Hts].
+      split; [split|].
+      - destruct HI as [Hρ [Hc [Hp Hor]]].
+        split; [exact Hρ|]. split; [eapply IConcrete_same; eauto|]. split.
+        + intros st0 t' x v Heq. apply Hts in Heq.
+          destruct (Hp _ _ _ _ Heq) as [l [r [Hl [Hx Hat]]]].
+          exists l, r. simpl. destruct Hsame as [Hr _]. rewrite Hr. auto.
+        + destruct Hor as [He|Hr]; [left; exact He|right; eapply Rep_same; eauto].
+      - apply (HP σ1 σ2 ρ1 π1); [apply same_heaps_grow; exact Hsame|exact Hpre].
+      - apply G_same; auto.
+    Qed.
+
+    (** Reading the record cell. *)
+    Lemma rec_read_res_update t l r (P : assertion) :
+      CI P ->
+      PUpdate (G t) {| te_tid := t; te_ev := ResEv (in_rec (oread l)) r |}
+        (I //\\ P) (I //\\ P //\\ RecIs l r).
+    Proof.
+      intros HP σ1 ρ1 π1 [HI Hpre] σ2 Hstep.
+      apply (step_rec t (ResEv (oread l) r)) in Hstep.
+      destruct Hstep as [Hs [H1 [H2 [H3 H4]]]].
+      destruct (omem_read_res_shape _ _ _ _ _ Hs) as [s [Hc [Hr Hc']]].
+      assert (Hsame : same_heaps σ1 σ2).
+      { apply same_heaps_control; [rewrite Hc, Hc'|rewrite H1|rewrite H2|rewrite H3|rewrite H4];
+          reflexivity. }
+      exists ρ1, π1. split; [apply rt_refl|]. split.
+      - split; [eapply I_same; eauto; apply no_new_ts_write_eq; exact H2|].
+        split; [apply (HP σ1 σ2 ρ1 π1); [apply same_heaps_grow; exact Hsame|exact Hpre]|].
+        unfold RecIs, rec_h. simpl. rewrite Hc'. exact Hr.
+      - apply G_same; auto.
+    Qed.
+
+    (** Linearizing an operation other than [nmsetTS] without touching the
+        heaps. *)
+    Lemma G_lin_same t (f : Sig.op (li_sig F)) (ret : Sig.ar f) c c' a
+        (p : tmap (@LinState (li_sig F))) :
+      same_heaps c c' -> TMap.find t p = Some (ls_inv f) ->
+      (forall l ts, f <> nmsetTS l ts) ->
+      G t (st c a p) (st c' a (lin_π t f ret p)).
+    Proof.
+      intros Hsame Hlin Hf. apply G_same; auto.
+      - intros t' Hne. rewrite lin_π_other; auto.
+      - intros l Hat _. exfalso.
+        destruct (AtSetTS_self _ _ _ _ Hlin Hat) as [ts Heq]. eapply Hf. exact Heq.
+    Qed.
+
+    Lemma I_lin_same t (f : Sig.op (li_sig F)) (ret : Sig.ar f) c c' a
+        (p : tmap (@LinState (li_sig F))) :
+      same_heaps c c' -> no_new_ts_write c c' -> TMap.find t p = Some (ls_inv f) ->
+      (forall l ts, f <> nmsetTS l ts) ->
+      I (st c a p) -> I (st c' a (lin_π t f ret p)).
+    Proof.
+      intros Hsame Hts Hlin Hf HI.
+      eapply I_same; [exact Hsame|exact Hts|apply AtSetTS_lin; auto|exact HI].
+    Qed.
+
+    (** Reading a field is the linearization point of the corresponding
+        [nmget*] operation: either the representation holds and the value read
+        is the abstract one, or the racy error is already reachable. *)
+    Lemma field_read_lin t (f : Sig.op (li_sig F)) (ret : Sig.ar f) l r σ1 σ2 h π1 :
+      same_heaps σ1 σ2 -> no_new_ts_write σ1 σ2 ->
+      I (st σ1 (Idle h) π1) -> TMap.find t π1 = Some (ls_inv f) ->
+      (forall l' ts, f <> nmsetTS l' ts) ->
+      rec_h σ1 l = Some r ->
+      (forall n, h l = Some n -> represents σ1 r n ->
+        StepNodeMem {| te_tid := t; te_ev := InvEv f |} h h /\
+        StepNodeMem {| te_tid := t; te_ev := ResEv f ret |} h h) ->
+      exists ρ' π', @poss_steps _ (li_lts F) (@PossOk _ (li_lts F) (Idle h) π1) (@PossOk _ (li_lts F) ρ' π') /\
+        DoneOrErr t f ret (st σ2 ρ' π') /\ G t (st σ1 (Idle h) π1) (st σ2 ρ' π').
+    Proof.
+      intros Hsame Hts HI Hlin Hf Hr Hstep.
+      pose proof HI as [_ [_ [_ Hor]]].
+      destruct Hor as [Herr | [_ Hsome]].
+      - exists (Idle h), π1. split; [apply rt_refl|]. split.
+        + right. split; [eapply I_same; eauto|exact Herr].
+        + apply G_same; auto.
+      - destruct (Hsome _ _ Hr) as [n [Hn Hrep]]. unfold abs in Hn. simpl in Hn.
+        destruct (Hstep _ Hn Hrep) as [Hinv Hres].
+        exists (Idle h), (lin_π t f ret π1). split.
+        + apply lin_steps; auto.
+        + split.
+          * left. split; [eapply I_lin_same; eauto|]. unfold ALin. simpl. apply lin_π_self.
+          * apply G_lin_same; auto.
+    Qed.
+
+    (** * Method: getValue *)
+
+    Lemma getValue_res_update t l lv lts lt ln v :
+      PUpdate (G t) {| te_tid := t; te_ev := ResEv (in_val (oread lv)) v |}
+        (Active t (nmgetValue l) //\\ RecIs l (mkrec lv lts lt ln))
+        (DoneOrErr t (nmgetValue l) v).
+    Proof.
+      intros σ1 ρ1 π1 [[HI Hlin] Hr] σ2 Hstep.
+      apply (step_val t (ResEv (oread lv) v)) in Hstep.
+      destruct Hstep as [Hs [H1 [H2 [H3 H4]]]].
+      destruct (omem_read_res_shape _ _ _ _ _ Hs) as [s [Hc [Hv Hc']]].
+      assert (Hsame : same_heaps σ1 σ2).
+      { apply same_heaps_control; [rewrite H1|rewrite Hc, Hc'|rewrite H2|rewrite H3|rewrite H4];
+          reflexivity. }
+      pose proof HI as [[h Hρ] _]. simpl in Hρ. subst ρ1.
+      eapply field_read_lin; eauto;
+        [apply no_new_ts_write_eq; exact H2|discriminate|].
+      intros [[[v0 ts0] tk0] nx0] Hn [Hval _]. simpl_fields Hval; simpl in Hval.
+      unfold val_h in Hval. rewrite Hc in Hval. simpl_fields Hval; simpl in Hval.
+      rewrite Hv in Hval. injection Hval as <-.
+      split.
+      - eapply step_getValue_inv; [reflexivity|rewrite Hn; discriminate].
+      - eapply step_getValue_res; [reflexivity|exact Hn].
+    Qed.
+
+    Lemma getValue_triple t l :
+      [li_lts E, li_lts F, lift_relation (R t), lift_relation (G t), lift_assert I, t] ⊢
+        {{ lift_assert (Active t (nmgetValue l)) }}
+          (@getValue_impl A l t)
+        {{ fun v => lift_assert (Done t (nmgetValue l) v) }}.
+    Proof.
+      eapply SetLogic.provable_perror.
+      { apply lift_perror. apply (defined_or_error t (nmgetValue l) l).
+        intros h Hnone. eapply error_getValue_undefined; [reflexivity|exact Hnone]. }
+      unfold getValue_impl.
+      eapply singleton_provable_vis_safe with
+        (P' := I //\\ (ALin t (ls_inv (nmgetValue l)) //\\ Defined l))
+        (Q' := fun r => I //\\ (ALin t (ls_inv (nmgetValue l)) //\\ Defined l) //\\ RecIs l r).
+      - apply read_rec_no_error. intros s [_ [_ H]]. exact H.
+      - intros s [HI _]. exact HI.
+      - intros r s [HI _]. exact HI.
+      - solve_conj_stable stableDB.
+      - intros r. solve_conj_stable stableDB.
+      - apply inv_update; [auto with ciDB|discriminate].
+      - intros r. apply rec_read_res_update. auto with ciDB.
+      - intros [[[lv lts] lt] ln]. cbn.
+        eapply singleton_provable_vis_safe with
+          (P' := Active t (nmgetValue l) //\\ RecIs l (mkrec lv lts lt ln))
+          (Q' := fun v => DoneOrErr t (nmgetValue l) v).
+        + apply (read_val_no_error t l (mkrec lv lts lt ln)).
+          intros s [HI [_ Hr]]. split; [exact HI|exact Hr].
+        + intros s [[HI _] _]. exact HI.
+        + intros v. apply DoneOrErr_I.
+        + solve_conj_stable stableDB.
+        + intros v. apply DoneOrErr_stable.
+        + eapply PUpdateConseq;
+            [apply ImplRefl| |apply inv_update; [auto with ciDB|discriminate]].
+          intros s [HI [[Hlin _] Hr]]. split; [split; [exact HI|exact Hlin]|exact Hr].
+        + intros v. apply getValue_res_update.
+        + intros v. eapply SetLogic.provable_perror; [apply DoneOrErr_perror|].
+          singleton_ret_safe; [apply ImplRefl|apply Done_I|apply Done_stable].
+    Qed.
+
+    (** * Methods: getTS, getTaken, getNext *)
+
+    Lemma getTS_res_update t l lv lts lt ln ts :
+      PUpdate (G t) {| te_tid := t; te_ev := ResEv (in_ts (oread lts)) ts |}
+        (Active t (nmgetTS l) //\\ RecIs l (mkrec lv lts lt ln))
+        (DoneOrErr t (nmgetTS l) ts).
+    Proof.
+      intros σ1 ρ1 π1 [[HI Hlin] Hr] σ2 Hstep.
+      apply (step_ts t (ResEv (oread lts) ts)) in Hstep.
+      destruct Hstep as [Hs [H1 [H2 [H3 H4]]]].
+      destruct (omem_read_res_shape _ _ _ _ _ Hs) as [s [Hc [Hv Hc']]].
+      assert (Hsame : same_heaps σ1 σ2).
+      { apply same_heaps_control; [rewrite H1|rewrite H2|rewrite Hc, Hc'|rewrite H3|rewrite H4];
+          reflexivity. }
+      pose proof HI as [[h Hρ] _]. simpl in Hρ. subst ρ1.
+      eapply field_read_lin; eauto;
+        [eapply no_new_ts_write_idle; exact Hc'|discriminate|].
+      intros [[[v0 ts0] tk0] nx0] Hn [_ [Hval _]]. simpl_fields Hval; simpl in Hval.
+      unfold ts_h in Hval. rewrite Hc in Hval. simpl_fields Hval; simpl in Hval.
+      rewrite Hv in Hval. injection Hval as <-.
+      split.
+      - eapply step_getTS_inv; [reflexivity|rewrite Hn; discriminate].
+      - eapply step_getTS_res; [reflexivity|exact Hn].
+    Qed.
+
+    Lemma getTS_triple t l :
+      [li_lts E, li_lts F, lift_relation (R t), lift_relation (G t), lift_assert I, t] ⊢
+        {{ lift_assert (Active t (nmgetTS l)) }}
+          (@getTS_impl A l t)
+        {{ fun v => lift_assert (Done t (nmgetTS l) v) }}.
+    Proof.
+      eapply SetLogic.provable_perror.
+      { apply lift_perror. apply (defined_or_error t (nmgetTS l) l).
+        intros h Hnone. eapply error_getTS_undefined; [reflexivity|exact Hnone]. }
+      unfold getTS_impl.
+      eapply singleton_provable_vis_safe with
+        (P' := I //\\ (ALin t (ls_inv (nmgetTS l)) //\\ Defined l))
+        (Q' := fun r => I //\\ (ALin t (ls_inv (nmgetTS l)) //\\ Defined l) //\\ RecIs l r).
+      - apply read_rec_no_error. intros s [_ [_ H]]. exact H.
+      - intros s [HI _]. exact HI.
+      - intros r s [HI _]. exact HI.
+      - solve_conj_stable stableDB.
+      - intros r. solve_conj_stable stableDB.
+      - apply inv_update; [auto with ciDB|discriminate].
+      - intros r. apply rec_read_res_update. auto with ciDB.
+      - intros [[[lv lts] lt] ln]. cbn.
+        eapply singleton_provable_vis_safe with
+          (P' := Active t (nmgetTS l) //\\ RecIs l (mkrec lv lts lt ln))
+          (Q' := fun v => DoneOrErr t (nmgetTS l) v).
+        + apply (read_ts_no_error t l (mkrec lv lts lt ln)).
+          intros s [HI [_ Hr]]. split; [exact HI|exact Hr].
+        + intros s [[HI _] _]. exact HI.
+        + intros v. apply DoneOrErr_I.
+        + solve_conj_stable stableDB.
+        + intros v. apply DoneOrErr_stable.
+        + eapply PUpdateConseq;
+            [apply ImplRefl| |apply inv_update; [auto with ciDB|discriminate]].
+          intros s [HI [[Hlin _] Hr]]. split; [split; [exact HI|exact Hlin]|exact Hr].
+        + intros v. apply getTS_res_update.
+        + intros v. eapply SetLogic.provable_perror; [apply DoneOrErr_perror|].
+          singleton_ret_safe; [apply ImplRefl|apply Done_I|apply Done_stable].
+    Qed.
+
+    Lemma getTaken_res_update t l lv lts lt ln tk :
+      PUpdate (G t) {| te_tid := t; te_ev := ResEv (in_taken (oread lt)) tk |}
+        (Active t (nmgetTaken l) //\\ RecIs l (mkrec lv lts lt ln))
+        (DoneOrErr t (nmgetTaken l) tk).
+    Proof.
+      intros σ1 ρ1 π1 [[HI Hlin] Hr] σ2 Hstep.
+      apply (step_taken t (ResEv (oread lt) tk)) in Hstep.
+      destruct Hstep as [Hs [H1 [H2 [H3 H4]]]].
+      destruct (omem_read_res_shape _ _ _ _ _ Hs) as [s [Hc [Hv Hc']]].
+      assert (Hsame : same_heaps σ1 σ2).
+      { apply same_heaps_control; [rewrite H1|rewrite H2|rewrite H3|rewrite H4|rewrite Hc, Hc'];
+          reflexivity. }
+      pose proof HI as [[h Hρ] _]. simpl in Hρ. subst ρ1.
+      eapply field_read_lin; eauto;
+        [apply no_new_ts_write_eq; exact H3|discriminate|].
+      intros [[[v0 ts0] tk0] nx0] Hn [_ [_ [Hval _]]]. simpl_fields Hval; simpl in Hval.
+      unfold taken_h in Hval. rewrite Hc in Hval. simpl_fields Hval; simpl in Hval.
+      rewrite Hv in Hval. injection Hval as <-.
+      split.
+      - eapply step_getTaken_inv; [reflexivity|rewrite Hn; discriminate].
+      - eapply step_getTaken_res; [reflexivity|exact Hn].
+    Qed.
+
+    Lemma getTaken_triple t l :
+      [li_lts E, li_lts F, lift_relation (R t), lift_relation (G t), lift_assert I, t] ⊢
+        {{ lift_assert (Active t (nmgetTaken l)) }}
+          (@getTaken_impl A l t)
+        {{ fun v => lift_assert (Done t (nmgetTaken l) v) }}.
+    Proof.
+      eapply SetLogic.provable_perror.
+      { apply lift_perror. apply (defined_or_error t (nmgetTaken l) l).
+        intros h Hnone. eapply error_getTaken_undefined; [reflexivity|exact Hnone]. }
+      unfold getTaken_impl.
+      eapply singleton_provable_vis_safe with
+        (P' := I //\\ (ALin t (ls_inv (nmgetTaken l)) //\\ Defined l))
+        (Q' := fun r => I //\\ (ALin t (ls_inv (nmgetTaken l)) //\\ Defined l) //\\ RecIs l r).
+      - apply read_rec_no_error. intros s [_ [_ H]]. exact H.
+      - intros s [HI _]. exact HI.
+      - intros r s [HI _]. exact HI.
+      - solve_conj_stable stableDB.
+      - intros r. solve_conj_stable stableDB.
+      - apply inv_update; [auto with ciDB|discriminate].
+      - intros r. apply rec_read_res_update. auto with ciDB.
+      - intros [[[lv lts] lt] ln]. cbn.
+        eapply singleton_provable_vis_safe with
+          (P' := Active t (nmgetTaken l) //\\ RecIs l (mkrec lv lts lt ln))
+          (Q' := fun v => DoneOrErr t (nmgetTaken l) v).
+        + apply (read_taken_no_error t l (mkrec lv lts lt ln)).
+          intros s [HI [_ Hr]]. split; [exact HI|exact Hr].
+        + intros s [[HI _] _]. exact HI.
+        + intros v. apply DoneOrErr_I.
+        + solve_conj_stable stableDB.
+        + intros v. apply DoneOrErr_stable.
+        + eapply PUpdateConseq;
+            [apply ImplRefl| |apply inv_update; [auto with ciDB|discriminate]].
+          intros s [HI [[Hlin _] Hr]]. split; [split; [exact HI|exact Hlin]|exact Hr].
+        + intros v. apply getTaken_res_update.
+        + intros v. eapply SetLogic.provable_perror; [apply DoneOrErr_perror|].
+          singleton_ret_safe; [apply ImplRefl|apply Done_I|apply Done_stable].
+    Qed.
+
+    Lemma getNext_res_update t l lv lts lt ln nx :
+      PUpdate (G t) {| te_tid := t; te_ev := ResEv (in_next (oread ln)) nx |}
+        (Active t (nmgetNext l) //\\ RecIs l (mkrec lv lts lt ln))
+        (DoneOrErr t (nmgetNext l) nx).
+    Proof.
+      intros σ1 ρ1 π1 [[HI Hlin] Hr] σ2 Hstep.
+      apply (step_next t (ResEv (oread ln) nx)) in Hstep.
+      destruct Hstep as [Hs [H1 [H2 [H3 H4]]]].
+      destruct (omem_read_res_shape _ _ _ _ _ Hs) as [s [Hc [Hv Hc']]].
+      assert (Hsame : same_heaps σ1 σ2).
+      { apply same_heaps_control; [rewrite H1|rewrite H2|rewrite H3|rewrite Hc, Hc'|rewrite H4];
+          reflexivity. }
+      pose proof HI as [[h Hρ] _]. simpl in Hρ. subst ρ1.
+      eapply field_read_lin; eauto;
+        [apply no_new_ts_write_eq; exact H3|discriminate|].
+      intros [[[v0 ts0] tk0] nx0] Hn [_ [_ [_ Hval]]]. simpl_fields Hval; simpl in Hval.
+      unfold next_h in Hval. rewrite Hc in Hval. simpl_fields Hval; simpl in Hval.
+      rewrite Hv in Hval. injection Hval as <-.
+      split.
+      - eapply step_getNext_inv; [reflexivity|rewrite Hn; discriminate].
+      - eapply step_getNext_res; [reflexivity|exact Hn].
+    Qed.
+
+    Lemma getNext_triple t l :
+      [li_lts E, li_lts F, lift_relation (R t), lift_relation (G t), lift_assert I, t] ⊢
+        {{ lift_assert (Active t (nmgetNext l)) }}
+          (@getNext_impl A l t)
+        {{ fun v => lift_assert (Done t (nmgetNext l) v) }}.
+    Proof.
+      eapply SetLogic.provable_perror.
+      { apply lift_perror. apply (defined_or_error t (nmgetNext l) l).
+        intros h Hnone. eapply error_getNext_undefined; [reflexivity|exact Hnone]. }
+      unfold getNext_impl.
+      eapply singleton_provable_vis_safe with
+        (P' := I //\\ (ALin t (ls_inv (nmgetNext l)) //\\ Defined l))
+        (Q' := fun r => I //\\ (ALin t (ls_inv (nmgetNext l)) //\\ Defined l) //\\ RecIs l r).
+      - apply read_rec_no_error. intros s [_ [_ H]]. exact H.
+      - intros s [HI _]. exact HI.
+      - intros r s [HI _]. exact HI.
+      - solve_conj_stable stableDB.
+      - intros r. solve_conj_stable stableDB.
+      - apply inv_update; [auto with ciDB|discriminate].
+      - intros r. apply rec_read_res_update. auto with ciDB.
+      - intros [[[lv lts] lt] ln]. cbn.
+        eapply singleton_provable_vis_safe with
+          (P' := Active t (nmgetNext l) //\\ RecIs l (mkrec lv lts lt ln))
+          (Q' := fun v => DoneOrErr t (nmgetNext l) v).
+        + apply (read_next_no_error t l (mkrec lv lts lt ln)).
+          intros s [HI [_ Hr]]. split; [exact HI|exact Hr].
+        + intros s [[HI _] _]. exact HI.
+        + intros v. apply DoneOrErr_I.
+        + solve_conj_stable stableDB.
+        + intros v. apply DoneOrErr_stable.
+        + eapply PUpdateConseq;
+            [apply ImplRefl| |apply inv_update; [auto with ciDB|discriminate]].
+          intros s [HI [[Hlin _] Hr]]. split; [split; [exact HI|exact Hlin]|exact Hr].
+        + intros v. apply getNext_res_update.
+        + intros v. eapply SetLogic.provable_perror; [apply DoneOrErr_perror|].
+          singleton_ret_safe; [apply ImplRefl|apply Done_I|apply Done_stable].
+    Qed.
+
+    (** * Updating one field cell of a published node *)
+
+    Lemma IConcrete_grow c c' :
+      rec_h c' = rec_h c ->
+      (forall a, val_h c a <> None -> val_h c' a <> None) ->
+      (forall a, ts_h c a <> None -> ts_h c' a <> None) ->
+      (forall a, taken_h c a <> None -> taken_h c' a <> None) ->
+      (forall a, next_h c a <> None -> next_h c' a <> None) ->
+      IConcrete c -> IConcrete c'.
+    Proof.
+      intros Hr Hv Ht Hk Hn [Hf Hinj]. split.
+      - intros l r Hl. rewrite Hr in Hl. destruct (Hf _ _ Hl) as [H1 [H2 [H3 H4]]].
+        unfold fields_defined. auto.
+      - intros l1 l2 r1 r2 H1 H2. rewrite Hr in H1, H2. eapply Hinj; eauto.
+    Qed.
+
+    (** Representation after storing [b] into the taken cell of node [l]. *)
+    Lemma Rep_update_taken c c' h p p' l r n b :
+      IConcrete c -> Rep (st c (Idle h) p) ->
+      rec_h c' = rec_h c -> val_h c' = val_h c -> ts_h c' = ts_h c ->
+      next_h c' = next_h c ->
+      taken_h c' = heap_update (rec_taken r) b (taken_h c) ->
+      rec_h c l = Some r -> h l = Some n ->
+      Rep (st c' (Idle (heap_update l
+        (mknode (node_val n) (node_ts n) b (node_next n)) h)) p').
+    Proof.
+      intros [_ Hinj] [Hnone Hsome] Hr Hv Ht Hn Hk Hl Hh.
+      unfold Rep, abs in *. simpl in *. rewrite Hr. split.
+      - intros l'. rewrite (heap_update_none_iff _ _ _ _ _ Hh). auto.
+      - intros l' r' Hl'. destruct (Nat.eq_dec l l') as [<-|Hne].
+        + rewrite Hl in Hl'. injection Hl' as <-.
+          destruct (Hsome _ _ Hl) as [n0 [Hn0 Hrep]]. rewrite Hh in Hn0.
+          injection Hn0 as <-.
+          eexists. split; [apply HeapUpdateSelf|].
+          destruct Hrep as [H1 [H2 [H3 H4]]].
+          unfold represents. rewrite Hv, Ht, Hn, Hk. simpl.
+          split; [exact H1|]. split; [exact H2|]. split; [apply HeapUpdateSelf|exact H4].
+        + destruct (Hsome _ _ Hl') as [n' [Hn' Hrep]].
+          exists n'. split; [rewrite HeapUpdateOther; auto|].
+          destruct Hrep as [H1 [H2 [H3 H4]]].
+          unfold represents. rewrite Hv, Ht, Hn, Hk.
+          split; [exact H1|]. split; [exact H2|]. split; [|exact H4].
+          rewrite HeapUpdateOther; [exact H3|].
+          destruct (Hinj _ _ _ _ Hl Hl' Hne) as [_ Hk']. exact Hk'.
+    Qed.
+
+    (** Representation after storing [ts] into the timestamp cell of node [l]. *)
+    Lemma Rep_update_ts c c' h p p' l r n ts :
+      IConcrete c -> Rep (st c (Idle h) p) ->
+      rec_h c' = rec_h c -> val_h c' = val_h c -> taken_h c' = taken_h c ->
+      next_h c' = next_h c ->
+      ts_h c' = heap_update (rec_ts r) ts (ts_h c) ->
+      rec_h c l = Some r -> h l = Some n ->
+      Rep (st c' (Idle (heap_update l
+        (mknode (node_val n) ts (node_taken n) (node_next n)) h)) p').
+    Proof.
+      intros [_ Hinj] [Hnone Hsome] Hr Hv Hk Hn Ht Hl Hh.
+      unfold Rep, abs in *. simpl in *. rewrite Hr. split.
+      - intros l'. rewrite (heap_update_none_iff _ _ _ _ _ Hh). auto.
+      - intros l' r' Hl'. destruct (Nat.eq_dec l l') as [<-|Hne].
+        + rewrite Hl in Hl'. injection Hl' as <-.
+          destruct (Hsome _ _ Hl) as [n0 [Hn0 Hrep]]. rewrite Hh in Hn0.
+          injection Hn0 as <-.
+          eexists. split; [apply HeapUpdateSelf|].
+          destruct Hrep as [H1 [H2 [H3 H4]]].
+          unfold represents. rewrite Hv, Hk, Hn, Ht. simpl.
+          split; [exact H1|]. split; [apply HeapUpdateSelf|]. split; [exact H3|exact H4].
+        + destruct (Hsome _ _ Hl') as [n' [Hn' Hrep]].
+          exists n'. split; [rewrite HeapUpdateOther; auto|].
+          destruct Hrep as [H1 [H2 [H3 H4]]].
+          unfold represents. rewrite Hv, Hk, Hn, Ht.
+          split; [exact H1|]. split; [|split; [exact H3|exact H4]].
+          rewrite HeapUpdateOther; [exact H2|].
+          destruct (Hinj _ _ _ _ Hl Hl' Hne) as [Ht' _]. exact Ht'.
+    Qed.
+
+    (** Heap rely after a store to a referenced taken cell. *)
+    Lemma HeapRely_update_taken c c' a b :
+      rec_h c' = rec_h c -> val_h c' = val_h c -> val_o c' = val_o c ->
+      ts_h c' = ts_h c -> ts_o c' = ts_o c -> taken_o c' = taken_o c ->
+      next_h c' = next_h c -> next_o c' = next_o c ->
+      taken_h c' = heap_update a b (taken_h c) ->
+      referenced_taken c a ->
+      HeapRely c c'.
+    Proof.
+      intros Hr Hv Hvo Ht Hto Hko Hn Hno Hk Href.
+      unfold HeapRely. rewrite Hr, Hv, Hvo, Ht, Hto, Hko, Hn, Hno, Hk.
+      repeat split; auto.
+      intros x v Hx Hnref. rewrite HeapUpdateOther; [exact Hx|].
+      intros <-. apply Hnref. exact Href.
+    Qed.
+
+    Lemma HeapRely_update_ts c c' a ts :
+      rec_h c' = rec_h c -> val_h c' = val_h c -> val_o c' = val_o c ->
+      taken_h c' = taken_h c -> taken_o c' = taken_o c -> ts_o c' = ts_o c ->
+      next_h c' = next_h c -> next_o c' = next_o c ->
+      ts_h c' = heap_update a ts (ts_h c) ->
+      referenced_ts c a ->
+      HeapRely c c'.
+    Proof.
+      intros Hr Hv Hvo Hk Hko Hto Hn Hno Ht Href.
+      unfold HeapRely. rewrite Hr, Hv, Hvo, Hk, Hko, Hto, Hn, Hno, Ht.
+      repeat split; auto.
+      intros x v Hx Hnref. rewrite HeapUpdateOther; [exact Hx|].
+      intros <-. apply Hnref. exact Href.
+    Qed.
+
+    (** * Method: tryTake *)
+
+    Lemma tryTake_read_res_update t l lv lts lt ln tk :
+      PUpdate (G t) {| te_tid := t; te_ev := ResEv (in_taken (oread lt)) tk |}
+        (Active t (nmtryTake l) //\\ RecIs l (mkrec lv lts lt ln))
+        (if tk then DoneOrErr t (nmtryTake l) false
+         else Active t (nmtryTake l) //\\ RecIs l (mkrec lv lts lt ln)).
+    Proof.
+      intros σ1 ρ1 π1 [[HI Hlin] Hr] σ2 Hstep.
+      apply (step_taken t (ResEv (oread lt) tk)) in Hstep.
+      destruct Hstep as [Hs [H1 [H2 [H3 H4]]]].
+      destruct (omem_read_res_shape _ _ _ _ _ Hs) as [s [Hc [Hv Hc']]].
+      assert (Hsame : same_heaps σ1 σ2).
+      { apply same_heaps_control; [rewrite H1|rewrite H2|rewrite H3|rewrite H4|rewrite Hc, Hc'];
+          reflexivity. }
+      destruct tk.
+      - pose proof HI as [[h Hρ] _]. simpl in Hρ. subst ρ1.
+        eapply field_read_lin; eauto;
+          [apply no_new_ts_write_eq; exact H3|discriminate|].
+        intros [[[v0 ts0] tk0] nx0] Hn [_ [_ [Hval _]]]. simpl_fields Hval; simpl in Hval.
+        unfold taken_h in Hval. rewrite Hc in Hval. simpl_fields Hval; simpl in Hval.
+        rewrite Hv in Hval. injection Hval as <-.
+        split.
+        + eapply step_tryTake_inv; [reflexivity|rewrite Hn; discriminate].
+        + eapply step_tryTake_res_fail; [reflexivity|exact Hn].
+      - exists ρ1, π1. split; [apply rt_refl|]. split.
+        + split; [split; [eapply I_same; eauto; apply no_new_ts_write_eq; exact H3|exact Hlin]|].
+          apply (RecIs_ci l (mkrec lv lts lt ln) σ1 σ2 ρ1 π1);
+            [apply same_heaps_grow; exact Hsame|exact Hr].
+        + apply G_same; auto.
+    Qed.
+
+    Lemma tryTake_cas_res_update t l lv lts lt ln b :
+      PUpdate (G t) {| te_tid := t; te_ev := ResEv (in_taken (ocas lt false true)) b |}
+        (Active t (nmtryTake l) //\\ RecIs l (mkrec lv lts lt ln))
+        (DoneOrErr t (nmtryTake l) b).
+    Proof.
+      intros σ1 ρ1 π1 [[HI Hlin] Hr] σ2 Hstep.
+      apply (step_taken t (ResEv (ocas lt false true) b)) in Hstep.
+      destruct Hstep as [Hs [H1 [H2 [H3 H4]]]].
+      pose proof HI as [[h Hρ] [Hcon [Hp Hor]]]. simpl in Hρ. subst ρ1.
+      unfold RecIs in Hr. simpl in Hr.
+      destruct b.
+      - destruct (omem_cas_true_shape _ _ _ _ _ _ Hs) as [s [Hc [Hv Hc']]].
+        assert (Hheaps : rec_h σ2 = rec_h σ1 /\ val_h σ2 = val_h σ1 /\
+          val_o σ2 = val_o σ1 /\ ts_h σ2 = ts_h σ1 /\ ts_o σ2 = ts_o σ1 /\
+          next_h σ2 = next_h σ1 /\ next_o σ2 = next_o σ1 /\
+          taken_o σ2 = taken_o σ1 /\ taken_h σ2 = heap_update lt true (taken_h σ1)).
+        { unfold rec_h, val_h, val_o, ts_h, ts_o, next_h, next_o, taken_o, taken_h.
+          rewrite H1, H2, H3, H4, Hc, Hc'. simpl. repeat split. }
+        destruct Hheaps as (Hr2 & Hv2 & Hvo2 & Ht2 & Hto2 & Hn2 & Hno2 & Hko2 & Hk2).
+        assert (Href : referenced_taken σ1 lt) by (exists l, (mkrec lv lts lt ln); auto).
+        assert (Hcon2 : IConcrete σ2).
+        { eapply IConcrete_grow; eauto; try (intros; congruence).
+          intros a Ha. rewrite Hk2. apply heap_update_defined. exact Ha. }
+        assert (HHR : HeapRely σ1 σ2).
+        { eapply HeapRely_update_taken; eauto. }
+        destruct Hor as [Herr | Hrep].
+        + exists (Idle h), π1. split; [apply rt_refl|]. split.
+          * right. split; [|exact Herr].
+            split; [eexists; reflexivity|]. split; [exact Hcon2|].
+            split; [eapply PendingTSWrite_same; eauto; apply no_new_ts_write_eq; exact H3|].
+            left. exact Herr.
+          * split; [auto|]. split; [exact HHR|].
+            split; [intros l0 r0 Ha Hb; simpl in Ha, Hb; rewrite Hr2 in Hb; congruence|]. split.
+            -- intros l0 n0 Hn0. exists n0. split; [exact Hn0|]. intros Hc0. contradiction.
+            -- auto.
+        + pose proof Hrep as [_ Hsome].
+          destruct (Hsome _ _ Hr) as [n [Hn Hrepn]]. unfold abs in Hn. simpl in Hn.
+          destruct n as [[[v0 ts0] tk0] nx0].
+          destruct Hrepn as [_ [_ [Hk _]]]. simpl_fields Hk; simpl in Hk.
+          unfold taken_h in Hk. rewrite Hc in Hk. simpl_fields Hk; simpl in Hk.
+          rewrite Hv in Hk. injection Hk as <-.
+          exists (Idle (heap_update l (mknode v0 ts0 true nx0) h)),
+            (lin_π t (nmtryTake l) true π1).
+          split.
+          * apply lin_steps; [exact Hlin| |].
+            -- eapply step_tryTake_inv; [reflexivity|rewrite Hn; discriminate].
+            -- eapply step_tryTake_res_succ; [reflexivity|exact Hn].
+          * split.
+            -- left. split; [|unfold ALin; simpl; apply lin_π_self].
+               split; [eexists; reflexivity|]. split; [exact Hcon2|]. split.
+               ++ eapply PendingTSWrite_same;
+                    [apply no_new_ts_write_eq; exact H3|exact Hr2
+                    |apply AtSetTS_lin; [exact Hlin|discriminate]|exact Hp].
+               ++ right.
+                  apply (Rep_update_taken σ1 σ2 h π1 _ l (mkrec lv lts lt ln)
+                    (mknode v0 ts0 false nx0) true); auto.
+            -- split; [intros t' Hne; simpl; rewrite lin_π_other; auto|].
+               split; [exact HHR|].
+               split; [intros l0 r0 Ha Hb; simpl in Ha, Hb; rewrite Hr2 in Hb; congruence|]. split.
+               ++ intros l0 n0 Hn0. unfold abs in Hn0. simpl in Hn0.
+                  destruct (Nat.eq_dec l l0) as [<-|Hne].
+                  ** exists (mknode v0 ts0 true nx0). split; [apply HeapUpdateSelf|].
+                     rewrite Hn in Hn0. injection Hn0 as <-. simpl. intros Hc0. contradiction.
+                  ** exists n0. split; [simpl_abs; rewrite HeapUpdateOther; auto|].
+                     intros Hc0. contradiction.
+               ++ intros l0 Hat _. exfalso.
+                  destruct (AtSetTS_self _ _ _ _ Hlin Hat) as [ts1 Heq]. discriminate Heq.
+      - destruct (omem_cas_false_shape _ _ _ _ _ _ Hs) as [s [u [Hc [Hu [Hne Hc']]]]].
+        destruct u; [|exfalso; apply Hne; reflexivity].
+        assert (Hsame : same_heaps σ1 σ2).
+        { apply same_heaps_control; [rewrite H1|rewrite H2|rewrite H3|rewrite H4|rewrite Hc, Hc'];
+            reflexivity. }
+        eapply field_read_lin; eauto;
+          [apply no_new_ts_write_eq; exact H3|discriminate|].
+        intros [[[v0 ts0] tk0] nx0] Hn [_ [_ [Hval _]]]. simpl_fields Hval; simpl in Hval.
+        unfold taken_h in Hval. rewrite Hc in Hval. simpl_fields Hval; simpl in Hval.
+        rewrite Hu in Hval. injection Hval as <-.
+        split.
+        + eapply step_tryTake_inv; [reflexivity|rewrite Hn; discriminate].
+        + eapply step_tryTake_res_fail; [reflexivity|exact Hn].
+    Qed.
+
+    Lemma tryTake_triple t l :
+      [li_lts E, li_lts F, lift_relation (R t), lift_relation (G t), lift_assert I, t] ⊢
+        {{ lift_assert (Active t (nmtryTake l)) }}
+          (@tryTake_impl A l t)
+        {{ fun b => lift_assert (Done t (nmtryTake l) b) }}.
+    Proof.
+      eapply SetLogic.provable_perror.
+      { apply lift_perror. apply (defined_or_error t (nmtryTake l) l).
+        intros h Hnone. eapply error_tryTake_undefined; [reflexivity|exact Hnone]. }
+      unfold tryTake_impl.
+      eapply singleton_provable_vis_safe with
+        (P' := I //\\ (ALin t (ls_inv (nmtryTake l)) //\\ Defined l))
+        (Q' := fun r => I //\\ (ALin t (ls_inv (nmtryTake l)) //\\ Defined l) //\\ RecIs l r).
+      - apply read_rec_no_error. intros s [_ [_ H]]. exact H.
+      - intros s [HI _]. exact HI.
+      - intros r s [HI _]. exact HI.
+      - solve_conj_stable stableDB.
+      - intros r. solve_conj_stable stableDB.
+      - apply inv_update; [auto with ciDB|discriminate].
+      - intros r. apply rec_read_res_update. auto with ciDB.
+      - intros [[[lv lts] lt] ln]. cbn.
+        eapply singleton_provable_vis_safe with
+          (P' := Active t (nmtryTake l) //\\ RecIs l (mkrec lv lts lt ln))
+          (Q' := fun tk : bool => if tk then DoneOrErr t (nmtryTake l) false
+                  else Active t (nmtryTake l) //\\ RecIs l (mkrec lv lts lt ln)).
+        + apply (read_taken_no_error t l (mkrec lv lts lt ln)).
+          intros s [HI [_ Hr]]. split; [exact HI|exact Hr].
+        + intros s [[HI _] _]. exact HI.
+        + intros [|]; [apply DoneOrErr_I|intros s [[HI _] _]; exact HI].
+        + solve_conj_stable stableDB.
+        + intros [|]; [apply DoneOrErr_stable|solve_conj_stable stableDB].
+        + eapply PUpdateConseq;
+            [apply ImplRefl| |apply inv_update; [auto with ciDB|discriminate]].
+          intros s [HI [[Hlin _] Hr]]. split; [split; [exact HI|exact Hlin]|exact Hr].
+        + intros tk. apply tryTake_read_res_update.
+        + intros [|].
+          * eapply SetLogic.provable_perror; [apply DoneOrErr_perror|].
+            singleton_ret_safe; [apply ImplRefl|apply Done_I|apply Done_stable].
+          * eapply singleton_provable_vis_safe with
+              (P' := Active t (nmtryTake l) //\\ RecIs l (mkrec lv lts lt ln))
+              (Q' := fun b => DoneOrErr t (nmtryTake l) b).
+            -- apply (cas_taken_no_error t l (mkrec lv lts lt ln)).
+               intros s [[HI _] Hr]. split; [exact HI|exact Hr].
+            -- intros s [[HI _] _]. exact HI.
+            -- intros b. apply DoneOrErr_I.
+            -- solve_conj_stable stableDB.
+            -- intros b. apply DoneOrErr_stable.
+            -- eapply PUpdateConseq;
+                 [| |apply (inv_update t _ (ALin t (ls_inv (nmtryTake l)) //\\
+                                            RecIs l (mkrec lv lts lt ln)));
+                     [auto with ciDB|discriminate]].
+               ++ intros s [[HI Hlin] Hr]. split; [exact HI|split; [exact Hlin|exact Hr]].
+               ++ intros s [HI [Hlin Hr]]. split; [split; [exact HI|exact Hlin]|exact Hr].
+            -- intros b. apply tryTake_cas_res_update.
+            -- intros b. eapply SetLogic.provable_perror; [apply DoneOrErr_perror|].
+               singleton_ret_safe; [apply ImplRefl|apply Done_I|apply Done_stable].
+    Qed.
+
+    (** * Method: setTS *)
+
+    (** Reading the timestamp cell.  [TSTop] records that the abstract
+        timestamp is still unset; an interval is the (no-op) linearization
+        point, unless another [setTS] on the node is in flight, in which case
+        the racy error is reachable and nothing is linearized. *)
+    Lemma setTS_read_res_update t l ts lv lts lt ln old :
+      PUpdate (G t) {| te_tid := t; te_ev := ResEv (in_ts (oread lts)) old |}
+        (Active t (nmsetTS l ts) //\\ RecIs l (mkrec lv lts lt ln))
+        (match old with
+         | TSTop => I //\\ TSTopSeen t l ts //\\ RecIs l (mkrec lv lts lt ln)
+         | TSInterval _ _ => DoneOrErr t (nmsetTS l ts) tt
+         end).
+    Proof.
+      intros σ1 ρ1 π1 [[HI Hlin] Hr] σ2 Hstep.
+      apply (step_ts t (ResEv (oread lts) old)) in Hstep.
+      destruct Hstep as [Hs [H1 [H2 [H3 H4]]]].
+      destruct (omem_read_res_shape _ _ _ _ _ Hs) as [s [Hc [Hv Hc']]].
+      assert (Hsame : same_heaps σ1 σ2).
+      { apply same_heaps_control; [rewrite H1|rewrite H2|rewrite Hc, Hc'|rewrite H3|rewrite H4];
+          reflexivity. }
+      assert (Hnw : no_new_ts_write σ1 σ2) by (eapply no_new_ts_write_idle; exact Hc').
+      pose proof HI as [[h Hρ] [Hcon [Hp Hor]]]. simpl in Hρ. subst ρ1.
+      unfold ALin in Hlin. simpl in Hlin. unfold RecIs in Hr. simpl in Hr.
+      assert (Hval : ts_h σ1 lts = Some old).
+      { unfold ts_h. rewrite Hc. simpl. exact Hv. }
+      destruct old as [|a b].
+      - (* TSTop *)
+        exists (Idle h), π1. split; [apply rt_refl|]. split.
+        + split; [eapply I_same; eauto|]. split; [|unfold RecIs; simpl; destruct Hsame as [Hr2 _]; rewrite Hr2; exact Hr].
+          split; [exact Hlin|].
+          destruct Hor as [Herr|[_ Hsome]]; [left; exact Herr|right].
+          destruct (Hsome _ _ Hr) as [n [Hn Hrep]]. exists n. split; [exact Hn|].
+          destruct Hrep as [_ [Ht _]]. simpl_fields Ht; simpl in Ht. rewrite Hval in Ht.
+          injection Ht as Ht. symmetry. exact Ht.
+        + apply G_same; auto.
+      - (* interval *)
+        destruct Hor as [Herr|Hrep].
+        + exists (Idle h), π1. split; [apply rt_refl|]. split.
+          * right. split; [eapply I_same; eauto|exact Herr].
+          * apply G_same; auto.
+        + destruct (classic (OtherAtSetTS (st σ1 (Idle h) π1) t l)) as [Hother|Hno].
+          * (* racing: the error is reachable, do not linearize *)
+            assert (Herr : Err (st σ1 (Idle h) π1)).
+            { destruct Hother as [t' [Hne Hat]]. exists l, t, t'. split; [exact Hne|].
+              split; [exists ts; exact Hlin|exact Hat]. }
+            exists (Idle h), π1. split; [apply rt_refl|]. split.
+            -- right. split; [eapply I_same; eauto|exact Herr].
+            -- apply G_same; auto.
+          * (* no-op linearization *)
+            pose proof Hrep as [_ Hsome].
+            destruct (Hsome _ _ Hr) as [n [Hn Hrep']]. unfold abs in Hn. simpl in Hn.
+            destruct n as [[[v0 ts0] tk0] nx0].
+            destruct Hrep' as [_ [Ht _]]. simpl_fields Ht; simpl in Ht. rewrite Hval in Ht.
+            injection Ht as <-.
+            change (h l = Some (mknode v0 (TSInterval a b) tk0 nx0)) in Hn.
+            exists (Idle (heap_update l (mknode v0 (TSInterval a b) tk0 nx0) h)),
+              (lin_π t (nmsetTS l ts) tt π1).
+            split.
+            { apply lin_steps; [exact Hlin| |].
+              - eapply step_setTS_inv; [reflexivity|rewrite Hn; discriminate].
+              - apply (step_setTS_res t h l v0 (TSInterval a b) tk0 nx0 ts);
+                  [reflexivity|exact Hn]. }
+            rewrite (heap_update_same h l _ Hn).
+            split.
+            -- left. split; [|unfold ALin; simpl; apply lin_π_self].
+               split; [eexists; reflexivity|]. split; [eapply IConcrete_same; eauto|].
+               split.
+               ++ intros st0 t' x v Hpend. simpl in Hpend. rewrite Hc' in Hpend. discriminate.
+               ++ right. eapply Rep_same; eauto.
+            -- apply G_same; auto.
+               ++ intros t' Hne. rewrite lin_π_other; auto.
+               ++ intros l0 Hat [t' [Hne Hat']]. exfalso. apply Hno.
+                  pose proof (AtSetTS_self_setTS _ _ _ _ _ Hlin Hat) as ->.
+                  exists t'. split; [exact Hne|exact Hat'].
+    Qed.
+
+    (** Invoking the store: the new pending store belongs to this [setTS]. *)
+    Lemma setTS_write_inv_update t l ts lv lts lt ln :
+      PUpdate (G t) {| te_tid := t; te_ev := InvEv (in_ts (owrite lts ts)) |}
+        (I //\\ TSTopSeen t l ts //\\ RecIs l (mkrec lv lts lt ln) //\\
+           NoOtherTSWrite t lts)
+        (I //\\ TSTopSeen t l ts //\\ RecIs l (mkrec lv lts lt ln)).
+    Proof.
+      intros σ1 ρ1 π1 [HI [Hseen [Hr _]]] σ2 Hstep.
+      apply (step_ts t (InvEv (owrite lts ts))) in Hstep.
+      destruct Hstep as [Hs [H1 [H2 [H3 H4]]]].
+      destruct (omem_inv_shape _ _ _ _ Hs) as [s [Hc Hc']].
+      assert (Hsame : same_heaps σ1 σ2).
+      { apply same_heaps_control; [rewrite H1|rewrite H2|rewrite Hc, Hc'|rewrite H3|rewrite H4];
+          reflexivity. }
+      exists ρ1, π1. split; [apply rt_refl|]. split.
+      - destruct HI as [Hρ [Hcon [Hp Hor]]].
+        split; [|split; [exact Hseen|apply (RecIs_ci l (mkrec lv lts lt ln) σ1 σ2 ρ1 π1);
+                                      [apply same_heaps_grow; exact Hsame|exact Hr]]].
+        split; [exact Hρ|]. split; [eapply IConcrete_same; eauto|]. split.
+        + intros st0 t' x v Hpend. simpl in Hpend. rewrite Hc' in Hpend.
+          injection Hpend as <- <- <- <-.
+          exists l, (mkrec lv lts lt ln). simpl.
+          destruct Hsame as [Hr2 _]. rewrite Hr2.
+          split; [exact Hr|]. split; [reflexivity|]. exists ts. apply Hseen.
+        + destruct Hor as [He|Hrep]; [left; exact He|right; eapply Rep_same; eauto].
+      - apply G_same; auto.
+    Qed.
+
+    (** The store's response: the linearization point of a [setTS] that found
+        [TSTop], unless another [setTS] on the node is in flight. *)
+    Lemma setTS_write_res_update t l ts lv lts lt ln :
+      PUpdate (G t) {| te_tid := t; te_ev := ResEv (in_ts (owrite lts ts)) tt |}
+        (I //\\ TSTopSeen t l ts //\\ RecIs l (mkrec lv lts lt ln))
+        (DoneOrErr t (nmsetTS l ts) tt).
+    Proof.
+      intros σ1 ρ1 π1 [HI [[Hlin Hseen] Hr]] σ2 Hstep.
+      apply (step_ts t (ResEv (owrite lts ts) tt)) in Hstep.
+      destruct Hstep as [Hs [H1 [H2 [H3 H4]]]].
+      destruct (omem_write_res_shape _ _ _ _ _ Hs) as [s [Hc [Hdef Hc']]].
+      pose proof HI as [[h Hρ] [Hcon [Hp Hor]]]. simpl in Hρ. subst ρ1.
+      simpl in Hlin. unfold RecIs in Hr. simpl in Hr.
+      assert (Hheaps : rec_h σ2 = rec_h σ1 /\ val_h σ2 = val_h σ1 /\
+        val_o σ2 = val_o σ1 /\ taken_h σ2 = taken_h σ1 /\ taken_o σ2 = taken_o σ1 /\
+        next_h σ2 = next_h σ1 /\ next_o σ2 = next_o σ1 /\
+        ts_o σ2 = ts_o σ1 /\ ts_h σ2 = heap_update lts ts (ts_h σ1)).
+      { unfold rec_h, val_h, val_o, ts_h, ts_o, next_h, next_o, taken_o, taken_h.
+        rewrite H1, H2, H3, H4, Hc, Hc'. simpl. repeat split. }
+      destruct Hheaps as (Hr2 & Hv2 & Hvo2 & Hk2 & Hko2 & Hn2 & Hno2 & Hto2 & Ht2).
+      assert (Href : referenced_ts σ1 lts) by (exists l, (mkrec lv lts lt ln); auto).
+      assert (Hcon2 : IConcrete σ2).
+      { eapply IConcrete_grow; eauto; try (intros; congruence).
+        intros a Ha. rewrite Ht2. apply heap_update_defined. exact Ha. }
+      assert (HHR : HeapRely σ1 σ2) by (eapply HeapRely_update_ts; eauto).
+      assert (Hnw : no_new_ts_write σ1 σ2) by (eapply no_new_ts_write_idle; exact Hc').
+      (* the branch that does not linearize *)
+      assert (Hstay : Err (st σ1 (Idle h) π1) ->
+        exists ρ' π', @poss_steps _ (li_lts F) (@PossOk _ (li_lts F) (Idle h) π1) (@PossOk _ (li_lts F) ρ' π') /\
+          DoneOrErr t (nmsetTS l ts) tt (st σ2 ρ' π') /\
+          G t (st σ1 (Idle h) π1) (st σ2 ρ' π')).
+      { intros Herr. exists (Idle h), π1. split; [apply rt_refl|]. split.
+        - right. split; [|exact Herr].
+          split; [eexists; reflexivity|]. split; [exact Hcon2|].
+          split; [eapply PendingTSWrite_same; eauto|left; exact Herr].
+        - split; [auto|]. split; [exact HHR|].
+          split; [intros l0 r0 Ha Hb; simpl in Ha, Hb; rewrite Hr2 in Hb; congruence|]. split.
+          + intros l0 n0 Hn0. exists n0. split; [exact Hn0|]. intros Hc0. contradiction.
+          + auto. }
+      destruct Hor as [Herr|Hrep]; [apply Hstay; exact Herr|].
+      destruct Hseen as [Herr|[n [Hn Htop]]]; [apply Hstay; exact Herr|].
+      destruct (classic (OtherAtSetTS (st σ1 (Idle h) π1) t l)) as [Hother|Hno].
+      { apply Hstay. destruct Hother as [t' [Hne Hat]]. exists l, t, t'.
+        split; [exact Hne|]. split; [exists ts; exact Hlin|exact Hat]. }
+      unfold abs in Hn. simpl in Hn.
+      destruct n as [[[v0 ts0] tk0] nx0]. simpl_fields Htop; simpl in Htop. subst ts0.
+      change (h l = Some (mknode v0 TSTop tk0 nx0)) in Hn.
+      exists (Idle (heap_update l (mknode v0 ts tk0 nx0) h)),
+        (lin_π t (nmsetTS l ts) tt π1).
+      split.
+      { apply lin_steps; [exact Hlin| |].
+        - eapply step_setTS_inv; [reflexivity|rewrite Hn; discriminate].
+        - apply (step_setTS_res t h l v0 TSTop tk0 nx0 ts); [reflexivity|exact Hn]. }
+      split.
+      - left. split; [|unfold ALin; simpl; apply lin_π_self].
+        split; [eexists; reflexivity|]. split; [exact Hcon2|]. split.
+        + intros st0 t' x v Hpend. simpl in Hpend. rewrite Hc' in Hpend. discriminate.
+        + right.
+          apply (Rep_update_ts σ1 σ2 h π1 _ l (mkrec lv lts lt ln)
+            (mknode v0 TSTop tk0 nx0) ts); auto.
+      - split; [intros t' Hne; simpl; rewrite lin_π_other; auto|].
+        split; [exact HHR|].
+        split; [intros l0 r0 Ha Hb; simpl in Ha, Hb; rewrite Hr2 in Hb; congruence|]. split.
+        + intros l0 n0 Hn0. unfold abs in Hn0. simpl in Hn0.
+          destruct (Nat.eq_dec l l0) as [<-|Hne].
+          * exists (mknode v0 ts tk0 nx0). split; [apply HeapUpdateSelf|].
+            intros _. exact Hno.
+          * exists n0. split; [simpl_abs; rewrite HeapUpdateOther; auto|].
+            intros Hc0. contradiction.
+        + intros l0 Hat [t' [Hne Hat']]. exfalso. apply Hno.
+          pose proof (AtSetTS_self_setTS _ _ _ _ _ Hlin Hat) as ->.
+          exists t'. split; [exact Hne|exact Hat'].
+    Qed.
+
+    Lemma setTS_triple t l ts :
+      [li_lts E, li_lts F, lift_relation (R t), lift_relation (G t), lift_assert I, t] ⊢
+        {{ lift_assert (Active t (nmsetTS l ts)) }}
+          (@setTS_impl A l ts t)
+        {{ fun u => lift_assert (Done t (nmsetTS l ts) u) }}.
+    Proof.
+      eapply SetLogic.provable_perror.
+      { apply lift_perror. apply (defined_or_error t (nmsetTS l ts) l).
+        intros h Hnone. eapply error_setTS_undefined; [reflexivity|exact Hnone]. }
+      unfold setTS_impl.
+      eapply singleton_provable_vis_safe with
+        (P' := I //\\ (ALin t (ls_inv (nmsetTS l ts)) //\\ Defined l))
+        (Q' := fun r => I //\\ (ALin t (ls_inv (nmsetTS l ts)) //\\ Defined l) //\\ RecIs l r).
+      - apply read_rec_no_error. intros s [_ [_ H]]. exact H.
+      - intros s [HI _]. exact HI.
+      - intros r s [HI _]. exact HI.
+      - solve_conj_stable stableDB.
+      - intros r. solve_conj_stable stableDB.
+      - apply inv_update; [auto with ciDB|discriminate].
+      - intros r. apply rec_read_res_update. auto with ciDB.
+      - intros [[[lv lts] lt] ln]. cbn.
+        eapply singleton_provable_vis_safe with
+          (P' := Active t (nmsetTS l ts) //\\ RecIs l (mkrec lv lts lt ln))
+          (Q' := fun old => match old with
+                  | TSTop => I //\\ TSTopSeen t l ts //\\ RecIs l (mkrec lv lts lt ln)
+                  | TSInterval _ _ => DoneOrErr t (nmsetTS l ts) tt
+                  end).
+        + apply (read_ts_no_error t l (mkrec lv lts lt ln)).
+          intros s [HI [_ Hr]]. split; [exact HI|exact Hr].
+        + intros s [[HI _] _]. exact HI.
+        + intros [|a b]; cbn beta iota; [intros s [HI _]; exact HI|apply DoneOrErr_I].
+        + solve_conj_stable stableDB.
+        + intros [|a b]; cbn beta iota; [solve_conj_stable stableDB|apply DoneOrErr_stable].
+        + eapply PUpdateConseq;
+            [apply ImplRefl| |apply inv_update; [auto with ciDB|discriminate]].
+          intros s [HI [[Hlin _] Hr]]. split; [split; [exact HI|exact Hlin]|exact Hr].
+        + intros old. apply setTS_read_res_update.
+        + intros [|a b]; cbn beta iota.
+          * (* TSTop: store the timestamp *)
+            eapply SetLogic.provable_perror.
+            { apply lift_perror. apply ts_write_race_or_error. }
+            eapply singleton_provable_vis_safe with
+              (P' := I //\\ TSTopSeen t l ts //\\ RecIs l (mkrec lv lts lt ln))
+              (Q' := fun _ => DoneOrErr t (nmsetTS l ts) tt).
+            -- apply (write_ts_no_error t l (mkrec lv lts lt ln)).
+            -- intros s [HI _]. exact HI.
+            -- intros u. apply DoneOrErr_I.
+            -- solve_conj_stable stableDB.
+            -- intros u. apply DoneOrErr_stable.
+            -- apply setTS_write_inv_update.
+            -- intros []. apply setTS_write_res_update.
+            -- intros []. eapply SetLogic.provable_perror; [apply DoneOrErr_perror|].
+               singleton_ret_safe; [apply ImplRefl|apply Done_I|apply Done_stable].
+          * eapply SetLogic.provable_perror; [apply DoneOrErr_perror|].
+            singleton_ret_safe; [apply ImplRefl|apply Done_I|apply Done_stable].
+    Qed.
+
+    (** * Method: malloc *)
+
+    Lemma Rep_grow c c' a p p' :
+      heaps_grow c c' -> Rep (st c a p) -> Rep (st c' a p').
+    Proof.
+      intros (Hr & Hv & _ & Ht & _ & Hk & _ & Hn & _) [H1 H2].
+      unfold Rep, represents, abs in *. simpl in *. rewrite Hr. split; [exact H1|].
+      intros l r Hl. destruct (H2 _ _ Hl) as [n [Hn' [Hv' [Ht' [Hk' Hn'']]]]].
+      exists n. split; [exact Hn'|]. split; [apply Hv; exact Hv'|].
+      split; [apply Ht; exact Ht'|]. split; [apply Hk; exact Hk'|apply Hn; exact Hn''].
+    Qed.
+
+    Lemma I_grow c c' a p :
+      heaps_grow c c' -> no_new_ts_write c c' -> I (st c a p) -> I (st c' a p).
+    Proof.
+      intros Hg Hnw [Hρ [Hc [Hp Hor]]].
+      split; [exact Hρ|]. split.
+      { cbn [st SinglePossState.σ] in Hc |- *.
+        destruct Hg as (Hr & Hv & _ & Ht & _ & Hk & _ & Hn & _).
+        eapply IConcrete_grow; eauto.
+        - intros x Hx. destruct (val_h c x) eqn:Hx'; [|contradiction]. rewrite (Hv _ _ Hx'). discriminate.
+        - intros x Hx. destruct (ts_h c x) eqn:Hx'; [|contradiction]. rewrite (Ht _ _ Hx'). discriminate.
+        - intros x Hx. destruct (taken_h c x) eqn:Hx'; [|contradiction]. rewrite (Hk _ _ Hx'). discriminate.
+        - intros x Hx. destruct (next_h c x) eqn:Hx'; [|contradiction]. rewrite (Hn _ _ Hx'). discriminate. }
+      split; [eapply PendingTSWrite_grow; eauto; destruct Hg as [Hr _]; intros l r; rewrite Hr; auto|].
+      destruct Hor as [He|Hrep]; [left; exact He|right; eapply Rep_grow; eauto].
+    Qed.
+
+    (** Allocating one field cell: the new cell is fresh and owned. *)
+    Lemma malloc_val_res_update t v lv (P : assertion) :
+      CI P ->
+      PUpdate (G t) {| te_tid := t; te_ev := ResEv (in_val (omalloc v)) lv |}
+        (I //\\ P) (I //\\ P //\\ FreshVal t lv v).
+    Proof.
+      intros HP σ1 ρ1 π1 [HI Hpre] σ2 Hstep.
+      apply (step_val t (ResEv (omalloc v) lv)) in Hstep.
+      destruct Hstep as [Hs [H1 [H2 [H3 H4]]]].
+      destruct (omem_alloc_res_shape _ _ _ _ _ Hs) as [s [Hc [Hnone Hc']]].
+      assert (Hheaps : rec_h σ2 = rec_h σ1 /\ ts_h σ2 = ts_h σ1 /\ ts_o σ2 = ts_o σ1 /\
+        taken_h σ2 = taken_h σ1 /\ taken_o σ2 = taken_o σ1 /\
+        next_h σ2 = next_h σ1 /\ next_o σ2 = next_o σ1 /\
+        val_h σ2 = heap_update lv v (val_h σ1) /\ val_o σ2 = heap_update lv t (val_o σ1) /\
+        val_h σ1 lv = None).
+      { unfold rec_h, val_h, val_o, ts_h, ts_o, next_h, next_o, taken_o, taken_h.
+        rewrite H1, H2, H3, H4, Hc, Hc'. simpl. repeat split. exact Hnone. }
+      destruct Hheaps as (Hr2 & Ht2 & Hto2 & Hk2 & Hko2 & Hn2 & Hno2 & Hv2 & Hvo2 & Hfresh).
+      assert (Hg : heaps_grow σ1 σ2).
+      { unfold heaps_grow. rewrite Hr2, Ht2, Hto2, Hk2, Hko2, Hn2, Hno2, Hv2, Hvo2.
+        split; [reflexivity|].
+        split; [intros a x Hx; apply heap_update_fresh; [exact Hfresh|exact Hx]|].
+        split; [intros a o Ha Ho; rewrite HeapUpdateOther; [exact Ho|];
+                intros <-; exact (Ha Hfresh)|].
+        repeat split; auto. }
+      exists ρ1, π1. split; [apply rt_refl|]. split.
+      - split; [eapply I_grow; eauto; apply no_new_ts_write_eq; exact H2|].
+        split; [apply (HP σ1 σ2 ρ1 π1); [exact Hg|exact Hpre]|].
+        unfold FreshVal. cbn [SinglePossState.σ].
+        split; [rewrite Hv2; apply HeapUpdateSelf|].
+        split; [rewrite Hvo2; apply HeapUpdateSelf|].
+        intros [l [r [Hl Hx]]]. rewrite Hr2 in Hl.
+        destruct HI as [_ [[Hf _] _]]. destruct (Hf _ _ Hl) as [Hd _].
+        cbn [SinglePossState.σ] in Hd. rewrite Hx in Hd. exact (Hd Hfresh).
+      - split; [auto|]. split.
+        { cbn [SinglePossState.σ]. unfold HeapRely. rewrite Hr2, Ht2, Hto2, Hk2, Hko2, Hn2, Hno2, Hv2, Hvo2.
+          repeat split; auto.
+          - intros a o Ha Ho. rewrite HeapUpdateOther; [exact Ho|]. intros <-. auto.
+          - intros a x Hx. apply heap_update_fresh; auto. }
+        split; [intros l0 r0 Ha Hb; simpl in Ha, Hb; rewrite Hr2 in Hb; congruence|]. split.
+        + intros l0 n0 Hn0. exists n0. split; [exact Hn0|]. intros Hc0. contradiction.
+        + auto.
+    Qed.
+
+    Lemma malloc_ts_res_update t lts (P : assertion) :
+      CI P ->
+      PUpdate (G t) {| te_tid := t; te_ev := ResEv (in_ts (omalloc TSTop)) lts |}
+        (I //\\ P) (I //\\ P //\\ FreshTS t lts).
+    Proof.
+      intros HP σ1 ρ1 π1 [HI Hpre] σ2 Hstep.
+      apply (step_ts t (ResEv (omalloc TSTop) lts)) in Hstep.
+      destruct Hstep as [Hs [H1 [H2 [H3 H4]]]].
+      destruct (omem_alloc_res_shape _ _ _ _ _ Hs) as [s [Hc [Hnone Hc']]].
+      assert (Hheaps : rec_h σ2 = rec_h σ1 /\ val_h σ2 = val_h σ1 /\ val_o σ2 = val_o σ1 /\
+        taken_h σ2 = taken_h σ1 /\ taken_o σ2 = taken_o σ1 /\
+        next_h σ2 = next_h σ1 /\ next_o σ2 = next_o σ1 /\
+        ts_h σ2 = heap_update lts TSTop (ts_h σ1) /\ ts_o σ2 = heap_update lts t (ts_o σ1) /\
+        ts_h σ1 lts = None).
+      { unfold rec_h, val_h, val_o, ts_h, ts_o, next_h, next_o, taken_o, taken_h.
+        rewrite H1, H2, H3, H4, Hc, Hc'. simpl. repeat split. exact Hnone. }
+      destruct Hheaps as (Hr2 & Hv2 & Hvo2 & Hk2 & Hko2 & Hn2 & Hno2 & Ht2 & Hto2 & Hfresh).
+      assert (Hg : heaps_grow σ1 σ2).
+      { unfold heaps_grow. rewrite Hr2, Hv2, Hvo2, Hk2, Hko2, Hn2, Hno2, Ht2, Hto2.
+        split; [reflexivity|]. split; [auto|]. split; [auto|].
+        split; [intros a x Hx; apply heap_update_fresh; [exact Hfresh|exact Hx]|].
+        split; [intros a o Ha Ho; rewrite HeapUpdateOther; [exact Ho|];
+                intros <-; exact (Ha Hfresh)|].
+        repeat split; auto. }
+      exists ρ1, π1. split; [apply rt_refl|]. split.
+      - split; [eapply I_grow; eauto; eapply no_new_ts_write_idle; exact Hc'|].
+        split; [apply (HP σ1 σ2 ρ1 π1); [exact Hg|exact Hpre]|].
+        unfold FreshTS. cbn [SinglePossState.σ].
+        split; [rewrite Ht2; apply HeapUpdateSelf|].
+        split; [rewrite Hto2; apply HeapUpdateSelf|].
+        intros [l [r [Hl Hx]]]. rewrite Hr2 in Hl.
+        destruct HI as [_ [[Hf _] _]]. destruct (Hf _ _ Hl) as [_ [Hd _]].
+        cbn [SinglePossState.σ] in Hd. rewrite Hx in Hd. exact (Hd Hfresh).
+      - split; [auto|]. split.
+        { cbn [SinglePossState.σ]. unfold HeapRely. rewrite Hr2, Hv2, Hvo2, Hk2, Hko2, Hn2, Hno2, Ht2, Hto2.
+          repeat split; auto.
+          - intros a o Ha Ho. rewrite HeapUpdateOther; [exact Ho|]. intros <-. auto.
+          - intros a x Hx _. apply heap_update_fresh; auto. }
+        split; [intros l0 r0 Ha Hb; simpl in Ha, Hb; rewrite Hr2 in Hb; congruence|]. split.
+        + intros l0 n0 Hn0. exists n0. split; [exact Hn0|]. intros Hc0. contradiction.
+        + auto.
+    Qed.
+
+    Lemma malloc_next_res_update t nx ln (P : assertion) :
+      CI P ->
+      PUpdate (G t) {| te_tid := t; te_ev := ResEv (in_next (omalloc nx)) ln |}
+        (I //\\ P) (I //\\ P //\\ FreshNext t ln nx).
+    Proof.
+      intros HP σ1 ρ1 π1 [HI Hpre] σ2 Hstep.
+      apply (step_next t (ResEv (omalloc nx) ln)) in Hstep.
+      destruct Hstep as [Hs [H1 [H2 [H3 H4]]]].
+      destruct (omem_alloc_res_shape _ _ _ _ _ Hs) as [s [Hc [Hnone Hc']]].
+      assert (Hheaps : rec_h σ2 = rec_h σ1 /\ val_h σ2 = val_h σ1 /\ val_o σ2 = val_o σ1 /\
+        taken_h σ2 = taken_h σ1 /\ taken_o σ2 = taken_o σ1 /\
+        ts_h σ2 = ts_h σ1 /\ ts_o σ2 = ts_o σ1 /\
+        next_h σ2 = heap_update ln nx (next_h σ1) /\ next_o σ2 = heap_update ln t (next_o σ1) /\
+        next_h σ1 ln = None).
+      { unfold rec_h, val_h, val_o, ts_h, ts_o, next_h, next_o, taken_o, taken_h.
+        rewrite H1, H2, H3, H4, Hc, Hc'. simpl. repeat split. exact Hnone. }
+      destruct Hheaps as (Hr2 & Hv2 & Hvo2 & Hk2 & Hko2 & Ht2 & Hto2 & Hn2 & Hno2 & Hfresh).
+      assert (Hg : heaps_grow σ1 σ2).
+      { unfold heaps_grow. rewrite Hr2, Hv2, Hvo2, Hk2, Hko2, Ht2, Hto2, Hn2, Hno2.
+        split; [reflexivity|]. split; [auto|]. split; [auto|]. split; [auto|].
+        split; [auto|]. split; [auto|]. split; [auto|].
+        split; [intros a x Hx; apply heap_update_fresh; [exact Hfresh|exact Hx]|].
+        intros a o Ha Ho; rewrite HeapUpdateOther; [exact Ho|];
+        intros <-; exact (Ha Hfresh). }
+      exists ρ1, π1. split; [apply rt_refl|]. split.
+      - split; [eapply I_grow; eauto; apply no_new_ts_write_eq; exact H3|].
+        split; [apply (HP σ1 σ2 ρ1 π1); [exact Hg|exact Hpre]|].
+        unfold FreshNext. cbn [SinglePossState.σ].
+        split; [rewrite Hn2; apply HeapUpdateSelf|].
+        split; [rewrite Hno2; apply HeapUpdateSelf|].
+        intros [l [r [Hl Hx]]]. rewrite Hr2 in Hl.
+        destruct HI as [_ [[Hf _] _]]. destruct (Hf _ _ Hl) as [_ [_ [_ Hd]]].
+        cbn [SinglePossState.σ] in Hd. rewrite Hx in Hd. exact (Hd Hfresh).
+      - split; [auto|]. split.
+        { cbn [SinglePossState.σ]. unfold HeapRely. rewrite Hr2, Hv2, Hvo2, Hk2, Hko2, Ht2, Hto2, Hn2, Hno2.
+          repeat split; auto.
+          - intros a o Ha Ho. rewrite HeapUpdateOther; [exact Ho|]. intros <-. auto.
+          - intros a x Hx. apply heap_update_fresh; auto. }
+        split; [intros l0 r0 Ha Hb; simpl in Ha, Hb; rewrite Hr2 in Hb; congruence|]. split.
+        + intros l0 n0 Hn0. exists n0. split; [exact Hn0|]. intros Hc0. contradiction.
+        + auto.
+    Qed.
+
+    Lemma malloc_taken_res_update t lt (P : assertion) :
+      CI P ->
+      PUpdate (G t) {| te_tid := t; te_ev := ResEv (in_taken (omalloc false)) lt |}
+        (I //\\ P) (I //\\ P //\\ FreshTaken t lt).
+    Proof.
+      intros HP σ1 ρ1 π1 [HI Hpre] σ2 Hstep.
+      apply (step_taken t (ResEv (omalloc false) lt)) in Hstep.
+      destruct Hstep as [Hs [H1 [H2 [H3 H4]]]].
+      destruct (omem_alloc_res_shape _ _ _ _ _ Hs) as [s [Hc [Hnone Hc']]].
+      assert (Hheaps : rec_h σ2 = rec_h σ1 /\ val_h σ2 = val_h σ1 /\ val_o σ2 = val_o σ1 /\
+        ts_h σ2 = ts_h σ1 /\ ts_o σ2 = ts_o σ1 /\
+        next_h σ2 = next_h σ1 /\ next_o σ2 = next_o σ1 /\
+        taken_h σ2 = heap_update lt false (taken_h σ1) /\
+        taken_o σ2 = heap_update lt t (taken_o σ1) /\
+        taken_h σ1 lt = None).
+      { unfold rec_h, val_h, val_o, ts_h, ts_o, next_h, next_o, taken_o, taken_h.
+        rewrite H1, H2, H3, H4, Hc, Hc'. simpl. repeat split. exact Hnone. }
+      destruct Hheaps as (Hr2 & Hv2 & Hvo2 & Ht2 & Hto2 & Hn2 & Hno2 & Hk2 & Hko2 & Hfresh).
+      assert (Hg : heaps_grow σ1 σ2).
+      { unfold heaps_grow. rewrite Hr2, Hv2, Hvo2, Ht2, Hto2, Hn2, Hno2, Hk2, Hko2.
+        split; [reflexivity|]. split; [auto|]. split; [auto|]. split; [auto|].
+        split; [auto|].
+        split; [intros a x Hx; apply heap_update_fresh; [exact Hfresh|exact Hx]|].
+        split; [intros a o Ha Ho; rewrite HeapUpdateOther; [exact Ho|];
+                intros <-; exact (Ha Hfresh)|].
+        split; auto. }
+      exists ρ1, π1. split; [apply rt_refl|]. split.
+      - split; [eapply I_grow; eauto; apply no_new_ts_write_eq; exact H3|].
+        split; [apply (HP σ1 σ2 ρ1 π1); [exact Hg|exact Hpre]|].
+        unfold FreshTaken. cbn [SinglePossState.σ].
+        split; [rewrite Hk2; apply HeapUpdateSelf|].
+        split; [rewrite Hko2; apply HeapUpdateSelf|].
+        intros [l [r [Hl Hx]]]. rewrite Hr2 in Hl.
+        destruct HI as [_ [[Hf _] _]]. destruct (Hf _ _ Hl) as [_ [_ [Hd _]]].
+        cbn [SinglePossState.σ] in Hd. rewrite Hx in Hd. exact (Hd Hfresh).
+      - split; [auto|]. split.
+        { cbn [SinglePossState.σ]. unfold HeapRely. rewrite Hr2, Hv2, Hvo2, Ht2, Hto2, Hn2, Hno2, Hk2, Hko2.
+          repeat split; auto.
+          - intros a o Ha Ho. rewrite HeapUpdateOther; [exact Ho|]. intros <-. auto.
+          - intros a x Hx _. apply heap_update_fresh; auto. }
+        split; [intros l0 r0 Ha Hb; simpl in Ha, Hb; rewrite Hr2 in Hb; congruence|]. split.
+        + intros l0 n0 Hn0. exists n0. split; [exact Hn0|]. intros Hc0. contradiction.
+        + auto.
+    Qed.
+
+    (** Representation after publishing a fresh record. *)
+    Lemma Rep_alloc c c' h p p' l r n :
+      Rep (st c (Idle h) p) ->
+      rec_h c' = heap_update l r (rec_h c) -> rec_h c l = None -> h l = None ->
+      val_h c' = val_h c -> ts_h c' = ts_h c -> taken_h c' = taken_h c ->
+      next_h c' = next_h c ->
+      represents c' r n ->
+      Rep (st c' (Idle (heap_update l n h)) p').
+    Proof.
+      intros [Hnone Hsome] Hr Hrl Hhl Hv Ht Hk Hn Hrep.
+      unfold Rep, abs in *. simpl in *. rewrite Hr. split.
+      - intros l'. destruct (Nat.eq_dec l l') as [<-|Hne].
+        + rewrite !HeapUpdateSelf. split; discriminate.
+        + rewrite !HeapUpdateOther; auto.
+      - intros l' r' Hl'. destruct (Nat.eq_dec l l') as [<-|Hne].
+        + rewrite HeapUpdateSelf in Hl'. injection Hl' as <-.
+          exists n. split; [apply HeapUpdateSelf|exact Hrep].
+        + rewrite HeapUpdateOther in Hl'; auto.
+          destruct (Hsome _ _ Hl') as [n' [Hn' Hrep']].
+          exists n'. split; [rewrite HeapUpdateOther; auto|].
+          unfold represents in *. rewrite Hv, Ht, Hk, Hn. exact Hrep'.
+    Qed.
+
+    Lemma malloc_rec_res_update t v nx lv lts lt ln l :
+      PUpdate (G t)
+        {| te_tid := t; te_ev := ResEv (in_rec (omalloc (mkrec lv lts lt ln))) l |}
+        (I //\\ ALin t (ls_inv (nmalloc v nx)) //\\ FreshVal t lv v //\\ FreshTS t lts
+           //\\ FreshNext t ln nx //\\ FreshTaken t lt)
+        (DoneOrErr t (nmalloc v nx) l).
+    Proof.
+      intros σ1 ρ1 π1 [HI [Hlin [Hfv [Hft [Hfn Hfk]]]]] σ2 Hstep.
+      apply (step_rec t (ResEv (omalloc (mkrec lv lts lt ln)) l)) in Hstep.
+      destruct Hstep as [Hs [H1 [H2 [H3 H4]]]].
+      destruct (omem_alloc_res_shape _ _ _ _ _ Hs) as [s [Hc [Hnone Hc']]].
+      pose proof HI as [[h Hρ] [Hcon [Hp Hor]]]. simpl in Hρ. subst ρ1.
+      simpl in Hlin.
+      destruct Hfv as [Hv1 [Hv2 Hv3]]. destruct Hft as [Ht1 [Ht2 Ht3]].
+      destruct Hfn as [Hn1 [Hn2 Hn3]]. destruct Hfk as [Hk1 [Hk2 Hk3]].
+      simpl in Hv1, Hv2, Hv3, Ht1, Ht2, Ht3, Hn1, Hn2, Hn3, Hk1, Hk2, Hk3.
+      assert (Hheaps : val_h σ2 = val_h σ1 /\ val_o σ2 = val_o σ1 /\
+        ts_h σ2 = ts_h σ1 /\ ts_o σ2 = ts_o σ1 /\
+        taken_h σ2 = taken_h σ1 /\ taken_o σ2 = taken_o σ1 /\
+        next_h σ2 = next_h σ1 /\ next_o σ2 = next_o σ1 /\
+        rec_h σ2 = heap_update l (mkrec lv lts lt ln) (rec_h σ1) /\ rec_h σ1 l = None).
+      { unfold rec_h, val_h, val_o, ts_h, ts_o, next_h, next_o, taken_o, taken_h.
+        rewrite H1, H2, H3, H4, Hc, Hc'. simpl. repeat split. exact Hnone. }
+      destruct Hheaps as (Hv2' & Hvo2 & Ht2' & Hto2 & Hk2' & Hko2 & Hn2' & Hno2 & Hr2 & Hrl).
+      assert (Hrec_old : forall l' r', rec_h σ1 l' = Some r' -> rec_h σ2 l' = Some r').
+      { intros l' r' Hl'. rewrite Hr2. apply heap_update_fresh; auto. }
+      assert (Hrec_new : forall l' r', rec_h σ2 l' = Some r' ->
+        (l' = l /\ r' = mkrec lv lts lt ln) \/ (l' <> l /\ rec_h σ1 l' = Some r')).
+      { intros l' r' Hl'. rewrite Hr2 in Hl'. destruct (Nat.eq_dec l l') as [<-|Hne].
+        - rewrite HeapUpdateSelf in Hl'. injection Hl' as <-. auto.
+        - rewrite HeapUpdateOther in Hl'; auto. }
+      assert (Hcon2 : IConcrete σ2).
+      { destruct Hcon as [Hf Hinj]. split.
+        - intros l' r' Hl'. destruct (Hrec_new _ _ Hl') as [[-> ->]|[_ Hold]].
+          + unfold fields_defined. rewrite Hv2', Ht2', Hk2', Hn2'. simpl_fields_goal.
+            repeat split; [rewrite Hv1|rewrite Ht1|rewrite Hk1|rewrite Hn1]; discriminate.
+          + destruct (Hf _ _ Hold) as [Ha [Hb [Hc0 Hd]]]. unfold fields_defined.
+            rewrite Hv2', Ht2', Hk2', Hn2'. auto.
+        - intros l1 l2 r1 r2 Hl1 Hl2 Hne.
+          destruct (Hrec_new _ _ Hl1) as [[-> ->]|[Hne1 Hold1]];
+          destruct (Hrec_new _ _ Hl2) as [[-> ->]|[Hne2 Hold2]].
+          + contradiction.
+          + simpl_fields_goal. split; intros Heq.
+            * apply Ht3. exists l2, r2. split; [exact Hold2|symmetry; exact Heq].
+            * apply Hk3. exists l2, r2. split; [exact Hold2|symmetry; exact Heq].
+          + simpl_fields_goal. split; intros Heq.
+            * apply Ht3. exists l1, r1. split; [exact Hold1|exact Heq].
+            * apply Hk3. exists l1, r1. split; [exact Hold1|exact Heq].
+          + eapply Hinj; eauto. }
+      assert (HHR : HeapRely σ1 σ2).
+      { unfold HeapRely. rewrite Hv2', Hvo2, Ht2', Hto2, Hk2', Hko2, Hn2', Hno2.
+        repeat split; auto. }
+      assert (Hnew : NewRecOwner (fun o => o = Some t) σ1 σ2).
+      { intros l' r' Hl1 Hl2. destruct (Hrec_new _ _ Hl2) as [[-> ->]|[_ Hold]];
+          [|congruence].
+        simpl_fields_goal. rewrite Hvo2, Hto2, Hko2, Hno2.
+        split; [exact Hv2|]. split; [exact Ht2|]. split; [exact Hk2|exact Hn2]. }
+      assert (Hpw : no_new_ts_write σ1 σ2) by (apply no_new_ts_write_eq; exact H2).
+      destruct Hor as [Herr|Hrep].
+      - exists (Idle h), π1. split; [apply rt_refl|]. split.
+        + right. split; [|exact Herr].
+          split; [eexists; reflexivity|]. split; [exact Hcon2|].
+          split; [eapply PendingTSWrite_grow; eauto|left; exact Herr].
+        + split; [auto|]. split; [exact HHR|]. split; [exact Hnew|]. split.
+          * intros l0 n0 Hn0. exists n0. split; [exact Hn0|]. intros Hc0. contradiction.
+          * auto.
+      - pose proof Hrep as [Hnone' _].
+        assert (Hhl : h l = None).
+        { apply Hnone'. exact Hrl. }
+        exists (Idle (heap_update l (mknode v TSTop false nx) h)),
+          (lin_π t (nmalloc v nx) l π1).
+        split.
+        { apply lin_steps; [exact Hlin| |].
+          - eapply step_malloc_inv; reflexivity.
+          - eapply step_malloc_res; [reflexivity|exact Hhl]. }
+        split.
+        + left. split; [|unfold ALin; simpl; apply lin_π_self].
+          split; [eexists; reflexivity|]. split; [exact Hcon2|]. split.
+          * eapply PendingTSWrite_grow;
+              [exact Hpw|exact Hrec_old|apply AtSetTS_lin; [exact Hlin|discriminate]|exact Hp].
+          * right. eapply Rep_alloc; eauto.
+            unfold represents. rewrite Hv2', Ht2', Hk2', Hn2'. simpl_fields_goal.
+            split; [exact Hv1|]. split; [exact Ht1|]. split; [exact Hk1|exact Hn1].
+        + split; [intros t' Hne; simpl; rewrite lin_π_other; auto|].
+          split; [exact HHR|]. split; [exact Hnew|]. split.
+          * intros l0 n0 Hn0. unfold abs in Hn0. simpl in Hn0.
+            exists n0. split; [|intros Hc0; contradiction].
+            simpl_abs. rewrite HeapUpdateOther; [exact Hn0|]. intros <-. congruence.
+          * intros l0 Hat _. exfalso.
+            destruct (AtSetTS_self _ _ _ _ Hlin Hat) as [ts' Heq]. discriminate Heq.
+    Qed.
+
+    Lemma malloc_triple t v nx :
+      [li_lts E, li_lts F, lift_relation (R t), lift_relation (G t), lift_assert I, t] ⊢
+        {{ lift_assert (Active t (nmalloc v nx)) }}
+          (@malloc_impl A v nx t)
+        {{ fun l => lift_assert (Done t (nmalloc v nx) l) }}.
+    Proof.
+      unfold malloc_impl.
+      eapply singleton_provable_vis_safe with
+        (P' := I //\\ ALin t (ls_inv (nmalloc v nx)))
+        (Q' := fun lv => I //\\ ALin t (ls_inv (nmalloc v nx)) //\\ FreshVal t lv v).
+      - apply alloc_val_no_error.
+      - intros s [HI _]. exact HI.
+      - intros lv s [HI _]. exact HI.
+      - solve_conj_stable stableDB.
+      - intros lv. solve_conj_stable stableDB.
+      - apply inv_update; [auto with ciDB|discriminate].
+      - intros lv. apply malloc_val_res_update. auto with ciDB.
+      - intros lv.
+        eapply singleton_provable_vis_safe with
+          (P' := I //\\ (ALin t (ls_inv (nmalloc v nx)) //\\ FreshVal t lv v))
+          (Q' := fun lts => I //\\ (ALin t (ls_inv (nmalloc v nx)) //\\ FreshVal t lv v)
+                           //\\ FreshTS t lts).
+        + apply alloc_ts_no_error.
+        + intros s [HI _]. exact HI.
+        + intros lts s [HI _]. exact HI.
+        + solve_conj_stable stableDB.
+        + intros lts. solve_conj_stable stableDB.
+        + apply inv_update; [auto with ciDB|discriminate].
+        + intros lts. apply malloc_ts_res_update. auto with ciDB.
+        + intros lts.
+          eapply singleton_provable_vis_safe with
+            (P' := I //\\ ((ALin t (ls_inv (nmalloc v nx)) //\\ FreshVal t lv v)
+                          //\\ FreshTS t lts))
+            (Q' := fun ln => I //\\ ((ALin t (ls_inv (nmalloc v nx)) //\\ FreshVal t lv v)
+                          //\\ FreshTS t lts) //\\ FreshNext t ln nx).
+          * apply alloc_next_no_error.
+          * intros s [HI _]. exact HI.
+          * intros ln s [HI _]. exact HI.
+          * solve_conj_stable stableDB.
+          * intros ln. solve_conj_stable stableDB.
+          * apply inv_update; [auto with ciDB|discriminate].
+          * intros ln. apply malloc_next_res_update. auto with ciDB.
+          * intros ln.
+            eapply singleton_provable_vis_safe with
+              (P' := I //\\ (((ALin t (ls_inv (nmalloc v nx)) //\\ FreshVal t lv v)
+                          //\\ FreshTS t lts) //\\ FreshNext t ln nx))
+              (Q' := fun lt => I //\\ (((ALin t (ls_inv (nmalloc v nx)) //\\ FreshVal t lv v)
+                          //\\ FreshTS t lts) //\\ FreshNext t ln nx) //\\ FreshTaken t lt).
+            -- apply alloc_taken_no_error.
+            -- intros s [HI _]. exact HI.
+            -- intros lt s [HI _]. exact HI.
+            -- solve_conj_stable stableDB.
+            -- intros lt. solve_conj_stable stableDB.
+            -- apply inv_update; [auto with ciDB|discriminate].
+            -- intros lt. apply malloc_taken_res_update. auto with ciDB.
+            -- intros lt.
+               eapply singleton_provable_vis_safe with
+                 (P' := I //\\ ALin t (ls_inv (nmalloc v nx)) //\\ FreshVal t lv v
+                          //\\ FreshTS t lts //\\ FreshNext t ln nx //\\ FreshTaken t lt)
+                 (Q' := fun l => DoneOrErr t (nmalloc v nx) l).
+               ++ apply alloc_rec_no_error.
+               ++ intros s [HI _]. exact HI.
+               ++ intros l. apply DoneOrErr_I.
+               ++ solve_conj_stable stableDB.
+               ++ intros l. apply DoneOrErr_stable.
+               ++ eapply PUpdateConseq; [|apply ImplRefl|apply inv_update; [auto with ciDB|discriminate]].
+                  intros s [HI [[[[Hlin Hfv] Hft] Hfn] Hfk]].
+                  split; [exact HI|]. split; [exact Hlin|]. split; [exact Hfv|].
+                  split; [exact Hft|]. split; [exact Hfn|exact Hfk].
+               ++ intros l. apply malloc_rec_res_update.
+               ++ intros l. eapply SetLogic.provable_perror; [apply DoneOrErr_perror|].
+                  singleton_ret_safe; [apply ImplRefl|apply Done_I|apply Done_stable].
+    Qed.
+
+    (** * The layer *)
+
+    Lemma I_ginv t f σ0 ρ0 π0 :
+      I (st σ0 ρ0 π0) -> TMap.find t π0 = None ->
+      I (st σ0 ρ0 (TMap.add t (ls_inv f) π0)).
+    Proof.
+      intros HI Hnone. eapply I_same; [| | |exact HI].
+      - unfold same_heaps. repeat split.
+      - apply no_new_ts_write_eq. reflexivity.
+      - intros t' l [ts Hat]. exists ts. rewrite TMap.gso; [exact Hat|].
+        intros <-. congruence.
+    Qed.
+
+    Lemma I_gret t f ret σ0 ρ0 π0 :
+      I (st σ0 ρ0 π0) -> TMap.find t π0 = Some (ls_linr f ret) ->
+      I (st σ0 ρ0 (TMap.remove t π0)).
+    Proof.
+      intros HI Hsome. eapply I_same; [| | |exact HI].
+      - unfold same_heaps. repeat split.
+      - apply no_new_ts_write_eq. reflexivity.
+      - intros t' l [ts Hat]. exists ts. rewrite TMap.gro; [exact Hat|].
+        intros <-. pose proof (eq_trans (eq_sym Hsome) Hat) as Heq. discriminate Heq.
+    Qed.
+
+    Lemma I_init :
+      I (st (li_init E) (li_init F) (TMap.empty _)).
+    Proof.
+      split; [eexists; reflexivity|]. split.
+      - split.
+        + intros l r Hl. discriminate.
+        + intros l1 l2 r1 r2 Hl. discriminate.
+      - split.
+        + intros st0 t' x v Hpend. discriminate.
+        + right. split.
+          * intros l. simpl. tauto.
+          * intros l r Hl. discriminate.
+    Qed.
+
+    Program Definition MNodeMem : layer_implementation_simulation E F :=
+    {| li_impl := @nodemem_impl A |}.
+    Next Obligation.
+      eapply SetLogic.soundness
+        with (R := fun t => lift_relation (R t))
+             (G := fun t => lift_relation (G t))
+             (I := lift_assert I).
+      (* valid RG *)
+      { intros t. eapply lift_valid_rgi. apply source_valid_rg. }
+      (* cross-thread compatibility *)
+      {
+        intros t1 t2 Hneq s s' Hrel.
+        eapply lift_parallel_compat; [exact Hneq| |exact Hrel].
+        apply source_rg_compatible; exact Hneq.
+      }
+      (* method provable *)
+      {
+        intros t f.
+        exists (lift_assert (Active t f)).
+        exists (fun ret => lift_assert (Done t f ret)).
+        constructor.
+        (* invocation *)
+        - intros s Hcompose.
+          eapply (lift_ginv_compose t f I (Active t f)); [|exact Hcompose].
+          intros out [pre [HI [Hσ [Hρ [Hnone Hπ]]]]].
+          destruct pre as [σp ρp πp], out as [σo ρo πo]. simpl in *. subst.
+          split.
+          + apply I_ginv; assumption.
+          + unfold ALin. simpl. apply PositiveMap.gss.
+        (* precondition entails invariant *)
+        - intros s Hlift. eapply lift_impl; [|exact Hlift]. apply Active_I.
+        (* precondition stable *)
+        - apply lift_stable. apply Active_stable.
+        (* return *)
+        - intros ret s Hcompose.
+          eapply (lift_gret_compose t f ret (Done t f ret) I); [|exact Hcompose].
+          intros out [pre [[HI Hlin] [Hσ [Hρ [Hsome Hπ]]]]].
+          destruct pre as [σp ρp πp], out as [σo ρo πo]. simpl in *. subst.
+          eapply I_gret; eassumption.
+        (* postcondition carries the linearized response *)
+        - intros ret σ0 Δ0 Hpost ρ0 π0 Hposs.
+          eapply (lift_post_lin (Done t f ret) t (ls_linr f ret));
+            [|exact Hpost|exact Hposs].
+          intros x [_ Hlin]. exact Hlin.
+        (* the method bodies *)
+        - destruct f; simpl.
+          + apply malloc_triple.
+          + apply setTS_triple.
+          + apply getValue_triple.
+          + apply getTS_triple.
+          + apply getTaken_triple.
+          + apply getNext_triple.
+          + apply tryTake_triple.
+      }
+      (* initial singleton *)
+      { apply lift_initial. apply I_init. }
+    Defined.
+
+    Definition MNodeMemLinearizable := LISim2LILin MNodeMem.
+
+    (** * Down to the concrete memories *)
+
+    (** The owner maps are ghost: [OwnerMemProof.MOwnerMem] realises each
+        [OwnerMem] over the plain memory with the same operations, so NodeMem
+        is linearizable from five concrete memories. *)
+    Definition EPlain : layer_interface :=
+      @PlainMemLayer.L (@NodeRec) ⊗ₗ @PlainMemLayer.L A ⊗ₗ @PlainMemLayer.L TS
+      ⊗ₗ @PlainMemLayer.L Ptr ⊗ₗ @PlainMemLayer.L bool.
+
+    Definition MNodeMemOverPlain :
+        layer_implementation_linearizability EPlain F :=
+      (⟦ @MOwnerMem (@NodeRec) ⟧ₗ ⊗ ⟦ @MOwnerMem A ⟧ₗ ⊗ ⟦ @MOwnerMem TS ⟧ₗ
+        ⊗ ⟦ @MOwnerMem Ptr ⟧ₗ ⊗ ⟦ @MOwnerMem bool ⟧ₗ) ▶ MNodeMemLinearizable.
+
+  End Proof.
+
+  Print Assumptions MNodeMem.
+  Print Assumptions MNodeMemOverPlain.
+
+End NodeMemProof.
